wip

Matroid/Matroid.lean
@@ -22,8 +22,8 @@ def Matroid.exists_maximal_subset_property {α : Type _} (P : Set α → Prop) (
 @[ext] structure Matroid (α : Type _) where
   (ground : Set α)
   (Base : Set α → Prop)
-  (exists_Base' : ∃ B, Base B)
-  (Base_exchange' : Matroid.exchange_property Base)
+  (exists_base' : ∃ B, Base B)
+  (base_exchange' : Matroid.exchange_property Base)
   (maximality' : ∀ X, X ⊆ ground → 
     Matroid.exists_maximal_subset_property (fun I ↦ ∃ B, Base B ∧ I ⊆ B) X)
   (subset_ground' : ∀ B, Base B → B ⊆ ground)
@@ -68,7 +68,7 @@ theorem encard_diff_eq_of_exch {Base : Set α → Prop} (exch : exchange_propert
 (encard_diff_le_aux exch hB₁ hB₂).antisymm (encard_diff_le_aux exch hB₂ hB₁)
 
 /-- Any two sets `B₁,B₂` in a family with the exchange property have the same `ℕ∞`-cardinality. -/
-theorem encard_Base_eq_of_exch {Base : Set α → Prop} (exch : exchange_property Base)
+theorem encard_base_eq_of_exch {Base : Set α → Prop} (exch : exchange_property Base)
     (hB₁ : Base B₁) (hB₂ : Base B₂) : B₁.encard = B₂.encard := by 
 rw [←encard_diff_add_encard_inter B₁ B₂, encard_diff_eq_of_exch exch hB₁ hB₂, inter_comm, 
      encard_diff_add_encard_inter]
@@ -82,13 +82,13 @@ def E (M : Matroid α) : Set α := M.ground
 
 @[simp] theorem ground_eq_E (M : Matroid α) : M.ground = M.E := rfl 
 
-/-- A set is Independent if it is contained in a Base.  -/
+/-- A set is independent if it is contained in a Base.  -/
 def Indep (M : Matroid α) (I : Set α) : Prop := ∃ B, M.Base B ∧ I ⊆ B
 
-/-- A subset of `M.E` is Dependent if it is not Independent . -/
+/-- A subset of `M.E` is Dependent if it is not independent . -/
 def Dep (M : Matroid α) (D : Set α) : Prop := ¬M.Indep D ∧ D ⊆ M.E   
 
-/-- A Basis for a set `X ⊆ M.E` is a maximal Independent subset of `X`
+/-- A Basis for a set `X ⊆ M.E` is a maximal independent subset of `X`
   (Often in the literature, the word 'Basis' is used to refer to what we call a 'Base'). -/
 def Basis (M : Matroid α) (I X : Set α) : Prop := 
   I ∈ maximals (· ⊆ ·) {A | M.Indep A ∧ A ⊆ X} ∧ X ⊆ M.E  
@@ -104,28 +104,28 @@ end defs
 /-- Typeclass for a matroid having finite ground set. This is just a wrapper for `[M.E.Finite]`-/
 class Finite (M : Matroid α) : Prop := (ground_finite : M.E.Finite)
 
-theorem ground_Finite (M : Matroid α) [M.Finite] : M.E.Finite := ‹M.Finite›.ground_finite   
+theorem ground_finite (M : Matroid α) [M.Finite] : M.E.Finite := ‹M.Finite›.ground_finite   
 
-theorem Set_Finite (M : Matroid α) [M.Finite] (X : Set α) (hX : X ⊆ M.E := by aesop) : X.Finite :=
-  M.ground_Finite.subset hX 
+theorem Set_finite (M : Matroid α) [M.Finite] (X : Set α) (hX : X ⊆ M.E := by aesop) : X.Finite :=
+  M.ground_finite.subset hX 
 
-instance Finite_of_Finite [@_root_.Finite α] {M : Matroid α} : Finite M := 
+instance finite_of_finite [@_root_.Finite α] {M : Matroid α} : Finite M := 
   ⟨Set.toFinite _⟩ 
 
-/-- A `Finite_rk` matroid is one with a finite Basis -/
-class Finite_rk (M : Matroid α) : Prop := (exists_finite_Base : ∃ B, M.Base B ∧ B.Finite) 
+/-- A `FiniteRk` matroid is one with a finite Basis -/
+class FiniteRk (M : Matroid α) : Prop := (exists_finite_base : ∃ B, M.Base B ∧ B.Finite) 
 
-instance Finite_rk_of_finite (M : Matroid α) [Finite M] : Finite_rk M := 
-  ⟨ M.exists_Base'.imp (fun B hB ↦ ⟨hB, M.Set_Finite B (M.subset_ground' _ hB)⟩) ⟩ 
+instance finiteRk_of_finite (M : Matroid α) [Finite M] : FiniteRk M := 
+  ⟨ M.exists_base'.imp (fun B hB ↦ ⟨hB, M.Set_finite B (M.subset_ground' _ hB)⟩) ⟩ 
 
-/-- An `Infinite_rk` matroid is one whose Bases are infinite. -/
-class Infinite_rk (M : Matroid α) : Prop := (exists_infinite_Base : ∃ B, M.Base B ∧ B.Infinite)
+/-- An `InfiniteRk` matroid is one whose Bases are infinite. -/
+class InfiniteRk (M : Matroid α) : Prop := (exists_infinite_base : ∃ B, M.Base B ∧ B.Infinite)
 
 /-- A `Finitary` matroid is one whose Circuits are finite -/
 class Finitary (M : Matroid α) : Prop := (cct_finite : ∀ (C : Set α), M.Circuit C → C.Finite) 
 
 /-- A `Rk_pos` matroid is one in which the empty set is not a Basis -/
-class Rk_pos (M : Matroid α) : Prop := (empty_not_Base : ¬M.Base ∅)
+class Rk_pos (M : Matroid α) : Prop := (empty_not_base : ¬M.Base ∅)
 
 section aesop
 
@@ -174,105 +174,105 @@ section Base
 theorem Base.subset_ground (hB : M.Base B) : B ⊆ M.E :=
   M.subset_ground' B hB 
 
-theorem exists_Base (M : Matroid α) : ∃ B, M.Base B := M.exists_Base'
+theorem exists_base (M : Matroid α) : ∃ B, M.Base B := M.exists_base'
 
 theorem Base.exchange (hB₁ : M.Base B₁) (hB₂ : M.Base B₂) (hx : e ∈ B₁ \ B₂) :
     ∃ y ∈ B₂ \ B₁, M.Base (insert y (B₁ \ {e}))  :=
-  M.Base_exchange' B₁ B₂ hB₁ hB₂ _ hx
+  M.base_exchange' B₁ B₂ hB₁ hB₂ _ hx
 
 theorem Base.exchange_mem (hB₁ : M.Base B₁) (hB₂ : M.Base B₂) (hxB₁ : e ∈ B₁) (hxB₂ : e ∉ B₂) :
     ∃ y, (y ∈ B₂ ∧ y ∉ B₁) ∧ M.Base (insert y (B₁ \ {e})) :=
   by simpa using hB₁.exchange hB₂ ⟨hxB₁, hxB₂⟩
 
-theorem Base.eq_of_subset_Base (hB₁ : M.Base B₁) (hB₂ : M.Base B₂) (hB₁B₂ : B₁ ⊆ B₂) :
+theorem Base.eq_of_subset_base (hB₁ : M.Base B₁) (hB₂ : M.Base B₂) (hB₁B₂ : B₁ ⊆ B₂) :
     B₁ = B₂ :=
-  antichain_of_exch M.Base_exchange' hB₁ hB₂ hB₁B₂
+  antichain_of_exch M.base_exchange' hB₁ hB₂ hB₁B₂
 
 theorem Base.encard_diff_comm (hB₁ : M.Base B₁) (hB₂ : M.Base B₂) :
     (B₁ \ B₂).encard = (B₂ \ B₁).encard :=
-  encard_diff_eq_of_exch (M.Base_exchange') hB₁ hB₂ 
+  encard_diff_eq_of_exch (M.base_exchange') hB₁ hB₂ 
 
 theorem Base.card_diff_comm (hB₁ : M.Base B₁) (hB₂ : M.Base B₂) :
     (B₁ \ B₂).ncard = (B₂ \ B₁).ncard := by
   rw [←encard_toNat_eq, hB₁.encard_diff_comm hB₂, encard_toNat_eq]
 
-theorem Base.encard_eq_encard_of_Base (hB₁ : M.Base B₁) (hB₂ : M.Base B₂) :
+theorem Base.encard_eq_encard_of_base (hB₁ : M.Base B₁) (hB₂ : M.Base B₂) :
     B₁.encard = B₂.encard := by
-  rw [encard_Base_eq_of_exch M.Base_exchange' hB₁ hB₂]
+  rw [encard_base_eq_of_exch M.base_exchange' hB₁ hB₂]
 
-theorem Base.card_eq_card_of_Base (hB₁ : M.Base B₁) (hB₂ : M.Base B₂) : B₁.ncard = B₂.ncard := by
-  rw [←encard_toNat_eq B₁, hB₁.encard_eq_encard_of_Base hB₂, encard_toNat_eq]
+theorem Base.card_eq_card_of_base (hB₁ : M.Base B₁) (hB₂ : M.Base B₂) : B₁.ncard = B₂.ncard := by
+  rw [←encard_toNat_eq B₁, hB₁.encard_eq_encard_of_base hB₂, encard_toNat_eq]
 
-theorem Base.Finite_of_Finite (hB : M.Base B) (h : B.Finite) (hB' : M.Base B') : B'.Finite :=
-  (Finite_iff_Finite_of_encard_eq_encard (hB.encard_eq_encard_of_Base hB')).mp h  
+theorem Base.finite_of_finite (hB : M.Base B) (h : B.Finite) (hB' : M.Base B') : B'.Finite :=
+  (finite_iff_finite_of_encard_eq_encard (hB.encard_eq_encard_of_base hB')).mp h  
 
-theorem Base.Infinite_of_Infinite (hB : M.Base B) (h : B.Infinite) (hB₁ : M.Base B₁) :
+theorem Base.infinite_of_infinite (hB : M.Base B) (h : B.Infinite) (hB₁ : M.Base B₁) :
     B₁.Infinite :=
-  by_contra (fun hB_inf ↦ (hB₁.Finite_of_Finite (not_infinite.mp hB_inf) hB).not_infinite h)
+  by_contra (fun hB_inf ↦ (hB₁.finite_of_finite (not_infinite.mp hB_inf) hB).not_infinite h)
 
-theorem Base.Finite [Finite_rk M] (hB : M.Base B) : B.Finite := 
-  let ⟨B₀,hB₀⟩ := ‹Finite_rk M›.exists_finite_Base
-  hB₀.1.Finite_of_Finite hB₀.2 hB
+theorem Base.finite [FiniteRk M] (hB : M.Base B) : B.Finite := 
+  let ⟨B₀,hB₀⟩ := ‹FiniteRk M›.exists_finite_base
+  hB₀.1.finite_of_finite hB₀.2 hB
 
-theorem Base.Infinite [Infinite_rk M] (hB : M.Base B) : B.Infinite :=
-  let ⟨B₀,hB₀⟩ := ‹Infinite_rk M›.exists_infinite_Base
-  hB₀.1.Infinite_of_Infinite hB₀.2 hB
+theorem Base.infinite [InfiniteRk M] (hB : M.Base B) : B.Infinite :=
+  let ⟨B₀,hB₀⟩ := ‹InfiniteRk M›.exists_infinite_base
+  hB₀.1.infinite_of_infinite hB₀.2 hB
 
-theorem Base.Finite_rk_of_Finite (hB : M.Base B) (hfin : B.Finite) : Finite_rk M := 
+theorem Base.finiteRk_of_finite (hB : M.Base B) (hfin : B.Finite) : FiniteRk M := 
   ⟨⟨B, hB, hfin⟩⟩   
 
-theorem Base.Infinite_rk_of_Infinite (hB : M.Base B) (h : B.Infinite) : Infinite_rk M := 
+theorem Base.infiniteRk_of_infinite (hB : M.Base B) (h : B.Infinite) : InfiniteRk M := 
   ⟨⟨B, hB, h⟩⟩ 
 
-theorem not_Finite_rk (M : Matroid α) [Infinite_rk M] : ¬ Finite_rk M := by
-  intro h; obtain ⟨B,hB⟩ := M.exists_Base; exact hB.Infinite hB.Finite
+theorem not_finiteRk (M : Matroid α) [InfiniteRk M] : ¬ FiniteRk M := by
+  intro h; obtain ⟨B,hB⟩ := M.exists_base; exact hB.infinite hB.finite
 
-theorem not_Infinite_rk (M : Matroid α) [Finite_rk M] : ¬ Infinite_rk M := by
-  intro h; obtain ⟨B,hB⟩ := M.exists_Base; exact hB.Infinite hB.Finite
+theorem not_infiniteRk (M : Matroid α) [FiniteRk M] : ¬ InfiniteRk M := by
+  intro h; obtain ⟨B,hB⟩ := M.exists_base; exact hB.infinite hB.finite
 
-theorem Finite_or_Infinite_rk (M : Matroid α) : Finite_rk M ∨ Infinite_rk M :=
-  let ⟨B, hB⟩ := M.exists_Base
+theorem finite_or_infiniteRk (M : Matroid α) : FiniteRk M ∨ InfiniteRk M :=
+  let ⟨B, hB⟩ := M.exists_base
   B.finite_or_infinite.elim 
-  (Or.inl ∘ hB.Finite_rk_of_Finite) (Or.inr ∘ hB.Infinite_rk_of_Infinite)
+  (Or.inl ∘ hB.finiteRk_of_finite) (Or.inr ∘ hB.infiniteRk_of_infinite)
 
-instance Finite_rk_of_Finite {M : Matroid α} [Finite M] : Finite_rk M := 
-  let ⟨B, hB⟩ := M.exists_Base
-  ⟨⟨B, hB, (M.ground_Finite).subset hB.subset_ground⟩⟩ 
+instance finite_rk_of_finite {M : Matroid α} [Finite M] : FiniteRk M := 
+  let ⟨B, hB⟩ := M.exists_base
+  ⟨⟨B, hB, (M.ground_finite).subset hB.subset_ground⟩⟩ 
 
-instance Finitary_of_Finite_rk {M : Matroid α} [Finite_rk M] : Finitary M := 
-⟨ by
+instance Finitary_of_FiniteRk {M : Matroid α} [FiniteRk M] : Finitary M := 
+⟨by {
   intros C hC
   obtain (rfl | ⟨e,heC⟩) := C.eq_empty_or_nonempty; exact finite_empty
   have hi : M.Indep (C \ {e}) :=
   by_contra (fun h ↦ (hC.2 ⟨h, (diff_subset _ _).trans hC.1.2⟩ (diff_subset C {e}) heC).2 rfl)
   obtain ⟨B, hB, hCB⟩ := hi 
-  convert (hB.Finite.subset hCB).insert e
-  rw [insert_diff_singleton, insert_eq_of_mem heC] ⟩  
+  convert (hB.finite.subset hCB).insert e
+  rw [insert_diff_singleton, insert_eq_of_mem heC] } ⟩  
 
 theorem Base.diff_finite_comm (hB₁ : M.Base B₁) (hB₂ : M.Base B₂) :
     (B₁ \ B₂).Finite ↔ (B₂ \ B₁).Finite := 
-  Finite_iff_Finite_of_encard_eq_encard (hB₁.encard_diff_comm hB₂)
+  finite_iff_finite_of_encard_eq_encard (hB₁.encard_diff_comm hB₂)
 
 theorem Base.diff_infinite_comm (hB₁ : M.Base B₁) (hB₂ : M.Base B₂) : 
     (B₁ \ B₂).Infinite ↔ (B₂ \ B₁).Infinite := 
-  Infinite_iff_Infinite_of_encard_eq_encard (hB₁.encard_diff_comm hB₂)
+  infinite_iff_infinite_of_encard_eq_encard (hB₁.encard_diff_comm hB₂)
 
-theorem Base.ncard_eq_ncard_of_Base (hB₁ : M.Base B₁) (hB₂ : M.Base B₂) : B₁.ncard = B₂.ncard :=
-by rw [←encard_toNat_eq, hB₁.encard_eq_encard_of_Base hB₂, encard_toNat_eq]
+theorem Base.ncard_eq_ncard_of_base (hB₁ : M.Base B₁) (hB₂ : M.Base B₂) : B₁.ncard = B₂.ncard :=
+by rw [←encard_toNat_eq, hB₁.encard_eq_encard_of_base hB₂, encard_toNat_eq]
 
-theorem eq_of_Base_iff_Base_forall {M₁ M₂ : Matroid α} (hE : M₁.E = M₂.E) 
+theorem eq_of_base_iff_base_forall {M₁ M₂ : Matroid α} (hE : M₁.E = M₂.E) 
     (h : ∀ B, B ⊆ M₁.E → (M₁.Base B ↔ M₂.Base B)) : M₁ = M₂ := by
   apply Matroid.ext _ _ hE
   ext B
   exact ⟨fun h' ↦ (h _ h'.subset_ground).mp h', 
     fun h' ↦ (h _ (h'.subset_ground.trans_eq hE.symm)).mpr h'⟩
 
-theorem Base_compl_iff_mem_maximals_disjoint_Base (hB : B ⊆ M.E := by aesop_mat) : 
+theorem base_compl_iff_mem_maximals_disjoint_base (hB : B ⊆ M.E := by aesop_mat) : 
     M.Base (M.E \ B) ↔ B ∈ maximals (· ⊆ ·) {I | I ⊆ M.E ∧ ∃ B, M.Base B ∧ Disjoint I B} := by
   simp_rw [mem_maximals_setOf_iff, and_iff_right hB, and_imp, forall_exists_index]
   refine' ⟨fun h ↦ ⟨⟨_, h, disjoint_sdiff_right⟩, 
     fun I hI B' ⟨hB', hIB'⟩ hBI ↦ hBI.antisymm _⟩, fun ⟨⟨ B', hB', hBB'⟩,h⟩ ↦ _⟩
-  · rw [hB'.eq_of_subset_Base h, ←subset_compl_iff_disjoint_right, diff_eq, compl_inter, 
+  · rw [hB'.eq_of_subset_base h, ←subset_compl_iff_disjoint_right, diff_eq, compl_inter, 
       compl_compl] at hIB'
     · exact fun e he ↦  (hIB' he).elim (fun h' ↦ (h' (hI he)).elim) id
     rw [subset_diff, and_iff_right hB'.subset_ground, disjoint_comm]
@@ -284,12 +284,11 @@ theorem Base_compl_iff_mem_maximals_disjoint_Base (hB : B ⊆ M.E := by aesop_ma
 
 end Base
 
+section dep_indep
 
-section Dep_Indep
+theorem indep_iff_subset_base : M.Indep I ↔ ∃ B, M.Base B ∧ I ⊆ B := Iff.rfl
 
-theorem Indep_iff_subset_Base : M.Indep I ↔ ∃ B, M.Base B ∧ I ⊆ B := Iff.rfl
-
-theorem Dep_iff : M.Dep D ↔ ¬M.Indep D ∧ D ⊆ M.E := Iff.rfl  
+theorem dep_iff : M.Dep D ↔ ¬M.Indep D ∧ D ⊆ M.E := Iff.rfl  
 
 @[aesop unsafe 15% (rule_sets [Matroid])]
 theorem Indep.subset_ground (hI : M.Indep I) : I ⊆ M.E := by 
@@ -304,29 +303,38 @@ theorem Dep.subset_ground (hD : M.Dep D) : D ⊆ M.E :=
 theorem Coindep.subset_ground (hX : M.Coindep X) : X ⊆ M.E :=
   hX.2
 
-theorem Indep_or_Dep (hX : X ⊆ M.E := by aesop_mat) : M.Indep X ∨ M.Dep X := by 
+theorem coindep_iff_exists (hX : X ⊆ M.E := by aesop_mat) : 
+    M.Coindep X ↔ ∃ B, M.Base B ∧ B ⊆ M.E \ X := by
+  simp_rw [Coindep, and_iff_left hX, subset_diff]
+  exact ⟨fun ⟨B, hB⟩ ↦ ⟨B, hB.1, hB.1.subset_ground, hB.2.symm⟩, 
+    fun ⟨B, hB⟩ ↦ ⟨B, hB.1, hB.2.2.symm⟩⟩
+
+theorem Coindep.exists_base_subset_compl (h : M.Coindep X) : ∃ B, M.Base B ∧ B ⊆ M.E \ X := 
+  (coindep_iff_exists h.subset_ground).mp h
+
+theorem indep_or_dep (hX : X ⊆ M.E := by aesop_mat) : M.Indep X ∨ M.Dep X := by 
   rw [Dep, and_iff_left hX]
   apply em
 
-theorem Indep.not_Dep (hI : M.Indep I) : ¬ M.Dep I := 
+theorem Indep.not_dep (hI : M.Indep I) : ¬ M.Dep I := 
   fun h ↦ h.1 hI   
 
-theorem Dep.not_Indep (hD : M.Dep D) : ¬ M.Indep D := 
+theorem Dep.not_indep (hD : M.Dep D) : ¬ M.Indep D := 
   hD.1  
 
-theorem Dep_of_not_Indep (hD : ¬ M.Indep D) (hDE : D ⊆ M.E := by aesop_mat) : M.Dep D := 
+theorem dep_of_not_indep (hD : ¬ M.Indep D) (hDE : D ⊆ M.E := by aesop_mat) : M.Dep D := 
   ⟨hD, hDE⟩ 
 
-theorem Indep_of_not_Dep (hI : ¬ M.Dep I) (hIE : I ⊆ M.E := by aesop_mat) : M.Indep I := 
+theorem indep_of_not_dep (hI : ¬ M.Dep I) (hIE : I ⊆ M.E := by aesop_mat) : M.Indep I := 
   by_contra (fun h ↦ hI ⟨h, hIE⟩)
 
-@[simp] theorem not_Dep_iff (hX : X ⊆ M.E := by aesop_mat) : ¬ M.Dep X ↔ M.Indep X := by
+@[simp] theorem not_dep_iff (hX : X ⊆ M.E := by aesop_mat) : ¬ M.Dep X ↔ M.Indep X := by
   rw [Dep, and_iff_left hX, not_not]
 
-@[simp] theorem not_Indep_iff (hX : X ⊆ M.E := by aesop_mat) : ¬ M.Indep X ↔ M.Dep X := by
+@[simp] theorem not_indep_iff (hX : X ⊆ M.E := by aesop_mat) : ¬ M.Indep X ↔ M.Dep X := by
   rw [Dep, and_iff_left hX]  
 
-theorem Indep.exists_Base_supset (hI : M.Indep I) : ∃ B, M.Base B ∧ I ⊆ B :=
+theorem Indep.exists_base_supset (hI : M.Indep I) : ∃ B, M.Base B ∧ I ⊆ B :=
   hI
 
 theorem Indep.subset (hJ : M.Indep J) (hIJ : I ⊆ J) : M.Indep I :=
@@ -334,14 +342,14 @@ theorem Indep.subset (hJ : M.Indep J) (hIJ : I ⊆ J) : M.Indep I :=
   ⟨B, hB, hIJ.trans hJB⟩
 
 theorem Dep.supset (hD : M.Dep D) (hDX : D ⊆ X) (hXE : X ⊆ M.E := by aesop_mat) : M.Dep X := 
-  Dep_of_not_Indep (fun hI ↦ (hI.subset hDX).not_Dep hD)
+  dep_of_not_indep (fun hI ↦ (hI.subset hDX).not_dep hD)
 
-@[simp] theorem empty_Indep (M : Matroid α) : M.Indep ∅ :=
-  Exists.elim M.exists_Base (fun B hB ↦ ⟨_, hB, B.empty_subset⟩)
+@[simp] theorem empty_indep (M : Matroid α) : M.Indep ∅ :=
+  Exists.elim M.exists_base (fun B hB ↦ ⟨_, hB, B.empty_subset⟩)
 
-theorem Indep.Finite [Finite_rk M] (hI : M.Indep I) : I.Finite := 
+theorem Indep.finite [FiniteRk M] (hI : M.Indep I) : I.Finite := 
   let ⟨_, hB, hIB⟩ := hI
-  hB.Finite.subset hIB  
+  hB.finite.subset hIB  
 
 theorem Indep.inter_right (hI : M.Indep I) (X : Set α) : M.Indep (I ∩ X) :=
   hI.subset (inter_subset_left _ _)
@@ -352,29 +360,29 @@ theorem Indep.inter_left (hI : M.Indep I) (X : Set α) : M.Indep (X ∩ I) :=
 theorem Indep.diff (hI : M.Indep I) (X : Set α) : M.Indep (I \ X) :=
   hI.subset (diff_subset _ _)
 
-theorem Base.Indep (hB : M.Base B) : M.Indep B :=
+theorem Base.indep (hB : M.Base B) : M.Indep B :=
   ⟨B, hB, subset_rfl⟩
 
-theorem Base.eq_of_subset_Indep (hB : M.Base B) (hI : M.Indep I) (hBI : B ⊆ I) : B = I :=
+theorem Base.eq_of_subset_indep (hB : M.Base B) (hI : M.Indep I) (hBI : B ⊆ I) : B = I :=
   let ⟨B', hB', hB'I⟩ := hI
-  hBI.antisymm (by rwa [hB.eq_of_subset_Base hB' (hBI.trans hB'I)])
+  hBI.antisymm (by rwa [hB.eq_of_subset_base hB' (hBI.trans hB'I)])
 
-theorem Base_iff_maximal_Indep : M.Base B ↔ M.Indep B ∧ ∀ I, M.Indep I → B ⊆ I → B = I := by
-  refine' ⟨fun h ↦ ⟨h.Indep, fun _ ↦ h.eq_of_subset_Indep ⟩, fun h ↦ _⟩
+theorem base_iff_maximal_indep : M.Base B ↔ M.Indep B ∧ ∀ I, M.Indep I → B ⊆ I → B = I := by
+  refine' ⟨fun h ↦ ⟨h.indep, fun _ ↦ h.eq_of_subset_indep ⟩, fun h ↦ _⟩
   obtain ⟨⟨B', hB', hBB'⟩, h⟩ := h
-  rwa [h _ hB'.Indep hBB']
+  rwa [h _ hB'.indep hBB']
 
-theorem Base_iff_mem_maximals : M.Base B ↔ B ∈ maximals (· ⊆ ·) {I | M.Indep I} := by
-  rw [Base_iff_maximal_Indep, mem_maximals_setOf_iff]
+theorem base_iff_mem_maximals : M.Base B ↔ B ∈ maximals (· ⊆ ·) {I | M.Indep I} := by
+  rw [base_iff_maximal_indep, mem_maximals_setOf_iff]
   
-theorem Indep.Base_of_maximal (hI : M.Indep I) (h : ∀ J, M.Indep J → I ⊆ J → I = J) : M.Base I := 
-  Base_iff_maximal_Indep.mpr ⟨hI,h⟩
+theorem Indep.base_of_maximal (hI : M.Indep I) (h : ∀ J, M.Indep J → I ⊆ J → I = J) : M.Base I := 
+  base_iff_maximal_indep.mpr ⟨hI,h⟩
 
-theorem Base.Dep_of_ssubset (hB : M.Base B) (h : B ⊂ X) (hX : X ⊆ M.E := by aesop_mat) : M.Dep X :=
-  ⟨λ hX ↦ h.ne (hB.eq_of_subset_Indep hX h.subset), hX⟩
+theorem Base.dep_of_ssubset (hB : M.Base B) (h : B ⊂ X) (hX : X ⊆ M.E := by aesop_mat) : M.Dep X :=
+  ⟨λ hX ↦ h.ne (hB.eq_of_subset_indep hX h.subset), hX⟩
 
-theorem Base.Dep_of_insert (hB : M.Base B) (heB : e ∉ B) (he : e ∈ M.E := by aesop_mat) : 
-    M.Dep (insert e B) := hB.Dep_of_ssubset (ssubset_insert heB)
+theorem Base.dep_of_insert (hB : M.Base B) (heB : e ∉ B) (he : e ∈ M.E := by aesop_mat) : 
+    M.Dep (insert e B) := hB.dep_of_ssubset (ssubset_insert heB)
 
 /-- If the difference of two Bases is a singleton, then they differ by an insertion/removal -/
 theorem Base.eq_exchange_of_diff_eq_singleton (hB : M.Base B) (hB' : M.Base B') (h : B \ B' = {e}) : 
@@ -382,11 +390,11 @@ theorem Base.eq_exchange_of_diff_eq_singleton (hB : M.Base B) (hB' : M.Base B') 
   obtain ⟨f, hf, hb⟩ := hB.exchange hB' (h.symm.subset (mem_singleton e))
   have hne : f ≠ e := by rintro rfl; exact hf.2 (h.symm.subset (mem_singleton f)).1
   rw [insert_diff_singleton_comm hne] at hb
-  refine ⟨f, hf, (hb.eq_of_subset_Base hB' ?_).symm⟩
+  refine ⟨f, hf, (hb.eq_of_subset_base hB' ?_).symm⟩
   rw [diff_subset_iff, insert_subset, union_comm, ←diff_subset_iff, h, and_iff_left rfl.subset]
   exact Or.inl hf.1
 
-theorem Base.exchange_Base_of_Indep (hB : M.Base B) (hf : f ∉ B) 
+theorem Base.exchange_base_of_indep (hB : M.Base B) (hf : f ∉ B) 
     (hI : M.Indep (insert f (B \ {e}))) : M.Base (insert f (B \ {e})) := by
   obtain ⟨B', hB', hIB'⟩ := hI
   have hcard := hB'.encard_diff_comm hB
@@ -401,17 +409,17 @@ theorem Base.exchange_Base_of_Indep (hB : M.Base B) (hf : f ∉ B)
     diff_union_inter]
   exact hB'
 
-theorem Base.exchange_Base_of_Indep' (hB : M.Base B) (he : e ∈ B) (hf : f ∉ B) 
+theorem Base.exchange_base_of_indep' (hB : M.Base B) (he : e ∈ B) (hf : f ∉ B) 
     (hI : M.Indep (insert f B \ {e})) : M.Base (insert f B \ {e}) := by
   have hfe : f ≠ e := by rintro rfl; exact hf he
   rw [←insert_diff_singleton_comm hfe] at *
-  exact hB.exchange_Base_of_Indep hf hI
+  exact hB.exchange_base_of_indep hf hI
 
-theorem Base.insert_Dep (hB : M.Base B) (h : e ∈ M.E \ B) : M.Dep (insert e B) := by
-  rw [←not_Indep_iff]
-  exact h.2 ∘ (fun hi ↦ insert_eq_self.mp (hB.eq_of_subset_Indep hi (subset_insert e B)).symm)
+theorem Base.insert_dep (hB : M.Base B) (h : e ∈ M.E \ B) : M.Dep (insert e B) := by
+  rw [←not_indep_iff]
+  exact h.2 ∘ (fun hi ↦ insert_eq_self.mp (hB.eq_of_subset_indep hi (subset_insert e B)).symm)
   
-theorem Indep.exists_insert_of_not_Base (hI : M.Indep I) (hI' : ¬M.Base I) (hB : M.Base B) : 
+theorem Indep.exists_insert_of_not_base (hI : M.Indep I) (hI' : ¬M.Base I) (hB : M.Base B) : 
     ∃ e ∈ B \ I, M.Indep (insert e I) := by
   obtain ⟨B', hB', hIB'⟩ := hI
   obtain ⟨x, hxB', hx⟩ := exists_of_ssubset (hIB'.ssubset_of_ne (by (rintro rfl; exact hI' hB'))) 
@@ -423,25 +431,25 @@ theorem Indep.exists_insert_of_not_Base (hI : M.Indep I) (hI' : ¬M.Base I) (hB 
 
 theorem Base.exists_insert_of_ssubset (hB : M.Base B) (hIB : I ⊂ B) (hB' : M.Base B') : 
   ∃ e ∈ B' \ I, M.Indep (insert e I) :=
-(hB.Indep.subset hIB.subset).exists_insert_of_not_Base 
-    (fun hI ↦ hIB.ne (hI.eq_of_subset_Base hB hIB.subset)) hB'
+(hB.indep.subset hIB.subset).exists_insert_of_not_base 
+    (fun hI ↦ hIB.ne (hI.eq_of_subset_base hB hIB.subset)) hB'
 
-theorem eq_of_Indep_iff_Indep_forall {M₁ M₂ : Matroid α} (hE : M₁.E = M₂.E) 
+theorem eq_of_indep_iff_indep_forall {M₁ M₂ : Matroid α} (hE : M₁.E = M₂.E) 
     (h : ∀ I, I ⊆ M₁.E → (M₁.Indep I ↔ M₂.Indep I)) : M₁ = M₂ :=
   let h' : ∀ I, M₁.Indep I ↔ M₂.Indep I := fun I ↦ 
     (em (I ⊆ M₁.E)).elim (h I) (fun h' ↦ iff_of_false (fun hi ↦ h' (hi.subset_ground)) 
       (fun hi ↦ h' (hi.subset_ground.trans_eq hE.symm)))
-  eq_of_Base_iff_Base_forall hE (fun B _ ↦ by simp_rw [Base_iff_maximal_Indep, h']) 
+  eq_of_base_iff_base_forall hE (fun B _ ↦ by simp_rw [base_iff_maximal_indep, h']) 
   
-theorem eq_iff_Indep_iff_Indep_forall {M₁ M₂ : Matroid α} : 
+theorem eq_iff_indep_iff_indep_forall {M₁ M₂ : Matroid α} : 
   M₁ = M₂ ↔ (M₁.E = M₂.E) ∧ ∀ I, I ⊆ M₁.E → (M₁.Indep I ↔ M₂.Indep I) :=
-⟨fun h ↦ by (subst h; simp), fun h ↦ eq_of_Indep_iff_Indep_forall h.1 h.2⟩  
+⟨fun h ↦ by (subst h; simp), fun h ↦ eq_of_indep_iff_indep_forall h.1 h.2⟩  
 
-end Dep_Indep
+end dep_indep
 
 section Basis
 
-theorem Basis.Indep (hI : M.Basis I X) : M.Indep I := hI.1.1.1
+theorem Basis.indep (hI : M.Basis I X) : M.Indep I := hI.1.1.1
 
 theorem Basis.subset (hI : M.Basis I X) : I ⊆ X := hI.1.1.2
 
@@ -449,204 +457,208 @@ theorem Basis.subset (hI : M.Basis I X) : I ⊆ X := hI.1.1.2
 theorem Basis.subset_ground (hI : M.Basis I X) : X ⊆ M.E :=
   hI.2 
 
-theorem Basis.Basis_inter_ground (hI : M.Basis I X) : M.Basis I (X ∩ M.E) := by
+theorem Basis.basis_inter_ground (hI : M.Basis I X) : M.Basis I (X ∩ M.E) := by
   convert hI
   rw [inter_eq_self_of_subset_left hI.subset_ground]
 
 @[aesop unsafe 15% (rule_sets [Matroid])]
 theorem Basis.left_subset_ground (hI : M.Basis I X) : I ⊆ M.E := 
-  hI.Indep.subset_ground
+  hI.indep.subset_ground
 
-theorem Basis.eq_of_subset_Indep (hI : M.Basis I X) (hJ : M.Indep J) (hIJ : I ⊆ J) (hJX : J ⊆ X) :
+theorem Basis.eq_of_subset_indep (hI : M.Basis I X) (hJ : M.Indep J) (hIJ : I ⊆ J) (hJX : J ⊆ X) :
     I = J :=
   hIJ.antisymm (hI.1.2 ⟨hJ, hJX⟩ hIJ)
 
-theorem Basis.Finite (hI : M.Basis I X) [Finite_rk M] : I.Finite := hI.Indep.Finite 
+theorem Basis.Finite (hI : M.Basis I X) [FiniteRk M] : I.Finite := hI.indep.finite 
 
-theorem Basis_iff' : 
+theorem basis_iff' : 
     M.Basis I X ↔ (M.Indep I ∧ I ⊆ X ∧ ∀ J, M.Indep J → I ⊆ J → J ⊆ X → I = J) ∧ X ⊆ M.E := by
   simp [Basis, mem_maximals_setOf_iff, and_assoc, and_congr_left_iff, and_imp, 
     and_congr_left_iff, and_congr_right_iff, @Imp.swap (_ ⊆ X)]
 
-theorem Basis_iff (hX : X ⊆ M.E := by aesop_mat) : 
+theorem basis_iff (hX : X ⊆ M.E := by aesop_mat) : 
   M.Basis I X ↔ (M.Indep I ∧ I ⊆ X ∧ ∀ J, M.Indep J → I ⊆ J → J ⊆ X → I = J) :=
-by rw [Basis_iff', and_iff_left hX]
+by rw [basis_iff', and_iff_left hX]
 
-theorem Basis_iff_mem_maximals (hX : X ⊆ M.E := by aesop_mat): 
+theorem basis_iff_mem_maximals (hX : X ⊆ M.E := by aesop_mat): 
     M.Basis I X ↔ I ∈ maximals (· ⊆ ·) {I | M.Indep I ∧ I ⊆ X} := by
   rw [Basis, and_iff_left hX]
 
-theorem Indep.Basis_of_maximal_subset (hI : M.Indep I) (hIX : I ⊆ X)
+theorem basis_iff_mem_maximals_Prop (hX : X ⊆ M.E := by aesop_mat): 
+    M.Basis I X ↔ I ∈ maximals (· ⊆ ·) (fun I ↦ M.Indep I ∧ I ⊆ X) :=
+  basis_iff_mem_maximals
+
+theorem Indep.basis_of_maximal_subset (hI : M.Indep I) (hIX : I ⊆ X)
     (hmax : ∀ ⦃J⦄, M.Indep J → I ⊆ J → J ⊆ X → J ⊆ I) (hX : X ⊆ M.E := by aesop_mat) : M.Basis I X := by
-  rw [Basis_iff (by aesop_mat : X ⊆ M.E), and_iff_right hI, and_iff_right hIX]
+  rw [basis_iff (by aesop_mat : X ⊆ M.E), and_iff_right hI, and_iff_right hIX]
   exact fun J hJ hIJ hJX ↦ hIJ.antisymm (hmax hJ hIJ hJX)
 
-theorem Basis.Basis_subset (hI : M.Basis I X) (hIY : I ⊆ Y) (hYX : Y ⊆ X) : M.Basis I Y := by
-  rw [Basis_iff (hYX.trans hI.subset_ground), and_iff_right hI.Indep, and_iff_right hIY] 
-  exact fun J hJ hIJ hJY ↦ hI.eq_of_subset_Indep hJ hIJ (hJY.trans hYX) 
+theorem Basis.basis_subset (hI : M.Basis I X) (hIY : I ⊆ Y) (hYX : Y ⊆ X) : M.Basis I Y := by
+  rw [basis_iff (hYX.trans hI.subset_ground), and_iff_right hI.indep, and_iff_right hIY] 
+  exact fun J hJ hIJ hJY ↦ hI.eq_of_subset_indep hJ hIJ (hJY.trans hYX) 
 
-@[simp] theorem Basis_self_iff_Indep : M.Basis I I ↔ M.Indep I := by
-  rw [Basis_iff', and_iff_right rfl.subset, and_assoc, and_iff_left_iff_imp] 
+@[simp] theorem basis_self_iff_indep : M.Basis I I ↔ M.Indep I := by
+  rw [basis_iff', and_iff_right rfl.subset, and_assoc, and_iff_left_iff_imp] 
   exact fun hi ↦ ⟨fun _ _ ↦ subset_antisymm, hi.subset_ground⟩ 
   
-theorem Indep.Basis_self (h : M.Indep I) : M.Basis I I :=
-  Basis_self_iff_Indep.mpr h
+theorem Indep.basis_self (h : M.Indep I) : M.Basis I I :=
+  basis_self_iff_indep.mpr h
 
-@[simp] theorem Basis_empty_iff (M : Matroid α) : M.Basis I ∅ ↔ I = ∅ :=
-  ⟨fun h ↦ subset_empty_iff.mp h.subset, fun h ↦ by (rw [h]; exact M.empty_Indep.Basis_self)⟩
+@[simp] theorem basis_empty_iff (M : Matroid α) : M.Basis I ∅ ↔ I = ∅ :=
+  ⟨fun h ↦ subset_empty_iff.mp h.subset, fun h ↦ by (rw [h]; exact M.empty_indep.basis_self)⟩
   
-theorem Basis.Dep_of_ssubset (hI : M.Basis I X) (hIY : I ⊂ Y) (hYX : Y ⊆ X) : M.Dep Y := by
+theorem Basis.dep_of_ssubset (hI : M.Basis I X) (hIY : I ⊂ Y) (hYX : Y ⊆ X) : M.Dep Y := by
   have : X ⊆ M.E := by aesop_mat 
-  rw [←not_Indep_iff]
-  exact fun hY ↦ hIY.ne (hI.eq_of_subset_Indep hY hIY.subset hYX)
+  rw [←not_indep_iff]
+  exact fun hY ↦ hIY.ne (hI.eq_of_subset_indep hY hIY.subset hYX)
 
-theorem Basis.insert_Dep (hI : M.Basis I X) (he : e ∈ X \ I) : M.Dep (insert e I) :=
-  hI.Dep_of_ssubset (ssubset_insert he.2) (insert_subset.mpr ⟨he.1,hI.subset⟩)
+theorem Basis.insert_dep (hI : M.Basis I X) (he : e ∈ X \ I) : M.Dep (insert e I) :=
+  hI.dep_of_ssubset (ssubset_insert he.2) (insert_subset.mpr ⟨he.1,hI.subset⟩)
 
-theorem Basis.mem_of_insert_Indep (hI : M.Basis I X) (he : e ∈ X) (hIe : M.Indep (insert e I)) : 
+theorem Basis.mem_of_insert_indep (hI : M.Basis I X) (he : e ∈ X) (hIe : M.Indep (insert e I)) : 
     e ∈ I :=
-  by_contra (fun heI ↦ (hI.insert_Dep ⟨he, heI⟩).not_Indep hIe) 
+  by_contra (fun heI ↦ (hI.insert_dep ⟨he, heI⟩).not_indep hIe) 
 
-theorem Basis.not_Basis_of_ssubset (hI : M.Basis I X) (hJI : J ⊂ I) : ¬ M.Basis J X :=
-  fun h ↦ hJI.ne (h.eq_of_subset_Indep hI.Indep hJI.subset hI.subset)
+theorem Basis.not_basis_of_ssubset (hI : M.Basis I X) (hJI : J ⊂ I) : ¬ M.Basis J X :=
+  fun h ↦ hJI.ne (h.eq_of_subset_indep hI.indep hJI.subset hI.subset)
 
-theorem Indep.subset_Basis_of_subset (hI : M.Indep I) (hIX : I ⊆ X) (hX : X ⊆ M.E := by aesop_mat) : 
+theorem Indep.subset_basis_of_subset (hI : M.Indep I) (hIX : I ⊆ X) (hX : X ⊆ M.E := by aesop_mat) : 
     ∃ J, M.Basis J X ∧ I ⊆ J := by
   obtain ⟨J, ⟨(hJ : M.Indep J),hIJ,hJX⟩, hJmax⟩ := M.maximality' X hX I hI hIX
   use J
-  rw [and_iff_left hIJ, Basis_iff, and_iff_right hJ, and_iff_right hJX]
+  rw [and_iff_left hIJ, basis_iff, and_iff_right hJ, and_iff_right hJX]
   exact fun K hK hJK hKX ↦ hJK.antisymm (hJmax ⟨hK, hIJ.trans hJK, hKX⟩ hJK)
 
-theorem exists_Basis (M : Matroid α) (X : Set α) (hX : X ⊆ M.E := by aesop_mat) :
+theorem exists_basis (M : Matroid α) (X : Set α) (hX : X ⊆ M.E := by aesop_mat) :
     ∃ I, M.Basis I X :=
-  let ⟨I, hI, _⟩ := M.empty_Indep.subset_Basis_of_subset (empty_subset X) 
+  let ⟨I, hI, _⟩ := M.empty_indep.subset_basis_of_subset (empty_subset X) 
   ⟨_,hI⟩
 
-theorem exists_Basis_subset_Basis (M : Matroid α) (hXY : X ⊆ Y) (hY : Y ⊆ M.E := by aesop_mat) :
+theorem exists_basis_subset_basis (M : Matroid α) (hXY : X ⊆ Y) (hY : Y ⊆ M.E := by aesop_mat) :
     ∃ I J, M.Basis I X ∧ M.Basis J Y ∧ I ⊆ J := by
-  obtain ⟨I, hI⟩ := M.exists_Basis X (hXY.trans hY)
-  obtain ⟨J, hJ, hIJ⟩ := hI.Indep.subset_Basis_of_subset (hI.subset.trans hXY)
+  obtain ⟨I, hI⟩ := M.exists_basis X (hXY.trans hY)
+  obtain ⟨J, hJ, hIJ⟩ := hI.indep.subset_basis_of_subset (hI.subset.trans hXY)
   exact ⟨_, _, hI, hJ, hIJ⟩ 
 
-theorem Basis.exists_Basis_inter_eq_of_supset (hI : M.Basis I X) (hXY : X ⊆ Y) 
+theorem Basis.exists_basis_inter_eq_of_supset (hI : M.Basis I X) (hXY : X ⊆ Y) 
     (hY : Y ⊆ M.E := by aesop_mat) : ∃ J, M.Basis J Y ∧ J ∩ X = I := by
-  obtain ⟨J, hJ, hIJ⟩ := hI.Indep.subset_Basis_of_subset (hI.subset.trans hXY)
+  obtain ⟨J, hJ, hIJ⟩ := hI.indep.subset_basis_of_subset (hI.subset.trans hXY)
   refine ⟨J, hJ, subset_antisymm ?_ (subset_inter hIJ hI.subset)⟩
-  exact fun e he ↦ hI.mem_of_insert_Indep he.2 (hJ.Indep.subset (insert_subset.mpr ⟨he.1, hIJ⟩))
+  exact fun e he ↦ hI.mem_of_insert_indep he.2 (hJ.indep.subset (insert_subset.mpr ⟨he.1, hIJ⟩))
 
-theorem exists_Basis_union_inter_Basis (M : Matroid α) (X Y : Set α) (hX : X ⊆ M.E := by aesop_mat) 
+theorem exists_basis_union_inter_basis (M : Matroid α) (X Y : Set α) (hX : X ⊆ M.E := by aesop_mat) 
     (hY : Y ⊆ M.E := by aesop_mat) : ∃ I, M.Basis I (X ∪ Y) ∧ M.Basis (I ∩ Y) Y :=
-  let ⟨J, hJ⟩ := M.exists_Basis Y
-  (hJ.exists_Basis_inter_eq_of_supset (subset_union_right X Y)).imp 
+  let ⟨J, hJ⟩ := M.exists_basis Y
+  (hJ.exists_basis_inter_eq_of_supset (subset_union_right X Y)).imp 
   (fun I hI ↦ ⟨hI.1, by rwa [hI.2]⟩)
 
-theorem Indep.eq_of_Basis (hI : M.Indep I) (hJ : M.Basis J I) : J = I :=
-  hJ.eq_of_subset_Indep hI hJ.subset rfl.subset
+theorem Indep.eq_of_basis (hI : M.Indep I) (hJ : M.Basis J I) : J = I :=
+  hJ.eq_of_subset_indep hI hJ.subset rfl.subset
 
-theorem Basis.exists_Base (hI : M.Basis I X) : ∃ B, M.Base B ∧ I = B ∩ X := 
-  let ⟨B,hB, hIB⟩ := hI.Indep
+theorem Basis.exists_base (hI : M.Basis I X) : ∃ B, M.Base B ∧ I = B ∩ X := 
+  let ⟨B,hB, hIB⟩ := hI.indep
   ⟨B, hB, subset_antisymm (subset_inter hIB hI.subset) 
-    (by rw [hI.eq_of_subset_Indep (hB.Indep.inter_right X) (subset_inter hIB hI.subset)
+    (by rw [hI.eq_of_subset_indep (hB.indep.inter_right X) (subset_inter hIB hI.subset)
     (inter_subset_right _ _)])⟩ 
 
-@[simp] theorem Basis_ground_iff : M.Basis B M.E ↔ M.Base B := by
-  rw [Base_iff_maximal_Indep, Basis_iff', and_assoc, and_congr_right]
+@[simp] theorem basis_ground_iff : M.Basis B M.E ↔ M.Base B := by
+  rw [base_iff_maximal_indep, basis_iff', and_assoc, and_congr_right]
   rw [and_iff_left (rfl.subset : M.E ⊆ M.E)]
   exact fun h ↦ ⟨fun h' I hI hBI ↦ h'.2 _ hI hBI hI.subset_ground,
     fun h' ↦ ⟨h.subset_ground,fun J hJ hBJ _ ↦ h' J hJ hBJ⟩⟩ 
 
-theorem Base.Basis_ground (hB : M.Base B) : M.Basis B M.E :=
-  Basis_ground_iff.mpr hB
+theorem Base.basis_ground (hB : M.Base B) : M.Basis B M.E :=
+  basis_ground_iff.mpr hB
 
-theorem Indep.Basis_of_forall_insert (hI : M.Indep I) (hIX : I ⊆ X) 
+theorem Indep.basis_of_forall_insert (hI : M.Indep I) (hIX : I ⊆ X) 
     (he : ∀ e ∈ X \ I, M.Dep (insert e I)) : M.Basis I X := by
-  rw [Basis_iff', and_iff_right hI, and_iff_right hIX]
+  rw [basis_iff', and_iff_right hI, and_iff_right hIX]
   refine' ⟨fun J hJ hIJ hJX ↦ hIJ.antisymm (fun e heJ ↦ by_contra (fun heI ↦ _)), 
     fun e heX ↦ (em (e ∈ I)).elim (fun h ↦ hI.subset_ground h) (fun heI ↦ _)⟩
-  · exact (he e ⟨(hJX heJ), heI⟩).not_Indep (hJ.subset (insert_subset.mpr ⟨heJ,hIJ⟩))
+  · exact (he e ⟨(hJX heJ), heI⟩).not_indep (hJ.subset (insert_subset.mpr ⟨heJ,hIJ⟩))
   exact (he e ⟨heX, heI⟩).subset_ground (mem_insert _ _)
     
-theorem Basis.iUnion_Basis_iUnion {ι : Type _} (X I : ι → Set α) (hI : ∀ i, M.Basis (I i) (X i)) 
+theorem Basis.iUnion_basis_iUnion {ι : Type _} (X I : ι → Set α) (hI : ∀ i, M.Basis (I i) (X i)) 
     (h_ind : M.Indep (⋃ i, I i)) : M.Basis (⋃ i, I i) (⋃ i, X i) := by
-  refine' h_ind.Basis_of_forall_insert 
+  refine' h_ind.basis_of_forall_insert 
     (iUnion_subset (fun i ↦ (hI i).subset.trans (subset_iUnion _ _))) _
   rintro e ⟨⟨_, ⟨⟨i, hi, rfl⟩, (hes : e ∈ X i)⟩⟩, he'⟩
   rw [mem_iUnion, not_exists] at he'
-  refine' ((hI i).insert_Dep ⟨hes, he' _⟩).supset (insert_subset_insert (subset_iUnion _ _)) _
+  refine' ((hI i).insert_dep ⟨hes, he' _⟩).supset (insert_subset_insert (subset_iUnion _ _)) _
   rw [insert_subset, iUnion_subset_iff, and_iff_left (by aesop_mat)]
   exact (hI i).subset_ground hes
 
-theorem Basis.Basis_iUnion {ι : Type _} [Nonempty ι] (X : ι → Set α) (hI : ∀ i, M.Basis I (X i)) : 
+theorem Basis.basis_iUnion {ι : Type _} [Nonempty ι] (X : ι → Set α) (hI : ∀ i, M.Basis I (X i)) : 
     M.Basis I (⋃ i, X i) := by
-  convert Basis.iUnion_Basis_iUnion X (fun _ ↦ I) (fun i ↦ hI i) _ <;> rw [iUnion_const]
-  exact (hI (Classical.arbitrary ι)).Indep
+  convert Basis.iUnion_basis_iUnion X (fun _ ↦ I) (fun i ↦ hI i) _ <;> rw [iUnion_const]
+  exact (hI (Classical.arbitrary ι)).indep
   
-theorem Basis.union_Basis_union (hIX : M.Basis I X) (hJY : M.Basis J Y) (h : M.Indep (I ∪ J)) : 
+theorem Basis.union_basis_union (hIX : M.Basis I X) (hJY : M.Basis J Y) (h : M.Indep (I ∪ J)) : 
     M.Basis (I ∪ J) (X ∪ Y) := by
   rw [union_eq_iUnion, union_eq_iUnion]
-  refine' Basis.iUnion_Basis_iUnion _ _ _ _
+  refine' Basis.iUnion_basis_iUnion _ _ _ _
   · simp only [Bool.forall_bool, cond_false, cond_true]; exact ⟨hJY, hIX⟩  
   rwa [←union_eq_iUnion]
   
-theorem Basis.Basis_union (hIX : M.Basis I X) (hIY : M.Basis I Y) : M.Basis I (X ∪ Y) := by
-    convert hIX.union_Basis_union hIY _ <;> rw [union_self]; exact hIX.Indep
+theorem Basis.basis_union (hIX : M.Basis I X) (hIY : M.Basis I Y) : M.Basis I (X ∪ Y) := by
+    convert hIX.union_basis_union hIY _ <;> rw [union_self]; exact hIX.indep
 
-theorem Basis.Basis_union_of_subset (hI : M.Basis I X) (hJ : M.Indep J) (hIJ : I ⊆ J) : 
+theorem Basis.basis_union_of_subset (hI : M.Basis I X) (hJ : M.Indep J) (hIJ : I ⊆ J) : 
     M.Basis J (J ∪ X) := by
-  convert hJ.Basis_self.union_Basis_union hI _ <;>
+  convert hJ.basis_self.union_basis_union hI _ <;>
   rw [union_eq_self_of_subset_right hIJ]
   assumption
 
-theorem Basis.insert_Basis_insert (hI : M.Basis I X) (h : M.Indep (insert e I)) : 
+theorem Basis.insert_basis_insert (hI : M.Basis I X) (h : M.Indep (insert e I)) : 
     M.Basis (insert e I) (insert e X) := by
   simp_rw [←union_singleton] at *
-  exact hI.union_Basis_union (h.subset (subset_union_right _ _)).Basis_self h
+  exact hI.union_basis_union (h.subset (subset_union_right _ _)).basis_self h
 
-theorem Base.Base_of_Basis_supset (hB : M.Base B) (hBX : B ⊆ X) (hIX : M.Basis I X) : M.Base I := by
+theorem Base.base_of_basis_supset (hB : M.Base B) (hBX : B ⊆ X) (hIX : M.Basis I X) : M.Base I := by
   by_contra h
-  obtain ⟨e,heBI,he⟩ := hIX.Indep.exists_insert_of_not_Base h hB
-  exact heBI.2 (hIX.mem_of_insert_Indep (hBX heBI.1) he)
+  obtain ⟨e,heBI,he⟩ := hIX.indep.exists_insert_of_not_base h hB
+  exact heBI.2 (hIX.mem_of_insert_indep (hBX heBI.1) he)
 
-theorem Indep.exists_Base_subset_union_Base (hI : M.Indep I) (hB : M.Base B) : 
+theorem Indep.exists_base_subset_union_base (hI : M.Indep I) (hB : M.Base B) : 
     ∃ B', M.Base B' ∧ I ⊆ B' ∧ B' ⊆ I ∪ B := by
-  obtain ⟨B', hB', hIB'⟩ := hI.subset_Basis_of_subset (subset_union_left I B)
-  exact ⟨B', hB.Base_of_Basis_supset (subset_union_right _ _) hB', hIB', hB'.subset⟩
+  obtain ⟨B', hB', hIB'⟩ := hI.subset_basis_of_subset (subset_union_left I B)
+  exact ⟨B', hB.base_of_basis_supset (subset_union_right _ _) hB', hIB', hB'.subset⟩
 
-theorem Basis.inter_eq_of_subset_Indep (hIX : M.Basis I X) (hIJ : I ⊆ J) (hJ : M.Indep J) : 
+theorem Basis.inter_eq_of_subset_indep (hIX : M.Basis I X) (hIJ : I ⊆ J) (hJ : M.Indep J) : 
   J ∩ X = I :=
 (subset_inter hIJ hIX.subset).antisymm' 
-  (fun _ he ↦ hIX.mem_of_insert_Indep he.2 (hJ.subset (insert_subset.mpr ⟨he.1, hIJ⟩))) 
+  (fun _ he ↦ hIX.mem_of_insert_indep he.2 (hJ.subset (insert_subset.mpr ⟨he.1, hIJ⟩))) 
 
-theorem Base.Basis_of_subset (hX : X ⊆ M.E := by aesop_mat) (hB : M.Base B) (hBX : B ⊆ X) : 
+theorem Base.basis_of_subset (hX : X ⊆ M.E := by aesop_mat) (hB : M.Base B) (hBX : B ⊆ X) : 
     M.Basis B X := by
-  rw [Basis_iff, and_iff_right hB.Indep, and_iff_right hBX]
-  exact fun J hJ hBJ _ ↦ hB.eq_of_subset_Indep hJ hBJ
+  rw [basis_iff, and_iff_right hB.indep, and_iff_right hBX]
+  exact fun J hJ hBJ _ ↦ hB.eq_of_subset_indep hJ hBJ
 
 end Basis
 section from_axioms
 
 /-- A constructor for matroids via the base axioms. 
   (In fact, just a wrapper for the definition of a matroid) -/
-def Matroid_of_Base (E : Set α) (Base : Set α → Prop) (exists_Base : ∃ B, Base B) 
-    (Base_exchange : exchange_property Base) 
+def matroid_of_base (E : Set α) (Base : Set α → Prop) (exists_base : ∃ B, Base B) 
+    (base_exchange : exchange_property Base) 
     (maximality : ∀ X, X ⊆ E → exists_maximal_subset_property (fun I ↦ ∃ B, Base B ∧ I ⊆ B) X)
     (support : ∀ B, Base B → B ⊆ E) : Matroid α := 
-  ⟨E, Base, exists_Base, Base_exchange, maximality, support⟩
+  ⟨E, Base, exists_base, base_exchange, maximality, support⟩
 
-@[simp] theorem Matroid_of_Base_apply (E : Set α) (Base : Set α → Prop) (exists_Base : ∃ B, Base B)
-    (Base_exchange : exchange_property Base) 
+@[simp] theorem matroid_of_base_apply (E : Set α) (Base : Set α → Prop) (exists_base : ∃ B, Base B)
+    (base_exchange : exchange_property Base) 
     (maximality : ∀ X, X ⊆ E → exists_maximal_subset_property (fun I ↦ ∃ B, Base B ∧ I ⊆ B) X)
     (support : ∀ B, Base B → B ⊆ E) : 
-    (Matroid_of_Base E Base exists_Base Base_exchange maximality support).Base = Base := rfl
+    (matroid_of_base E Base exists_base base_exchange maximality support).Base = Base := rfl
 
-/-- A version of the Independence axioms that avoids cardinality -/
-def Matroid_of_Indep (E : Set α) (Indep : Set α → Prop) (h_empty : Indep ∅) 
+/-- A version of the independence axioms that avoids cardinality -/
+def matroid_of_indep (E : Set α) (Indep : Set α → Prop) (h_empty : Indep ∅) 
     (h_subset : ∀ ⦃I J⦄, Indep J → I ⊆ J → Indep I) 
     (h_aug : ∀⦃I B⦄, Indep I → I ∉ maximals (· ⊆ ·) Indep → B ∈ maximals (· ⊆ ·) Indep → 
       ∃ x ∈ B \ I, Indep (insert x I))
     (h_maximal : ∀ X, X ⊆ E → exists_maximal_subset_property Indep X) 
     (h_support : ∀ I, Indep I → I ⊆ E) : Matroid α :=
-  Matroid_of_Base E (· ∈ maximals (· ⊆ ·) Indep)
+  matroid_of_base E (· ∈ maximals (· ⊆ ·) Indep)
   ( by 
       obtain ⟨B, ⟨hB,-,-⟩, hB₁⟩ := h_maximal E rfl.subset ∅ h_empty (empty_subset _)
       exact ⟨B, ⟨hB, fun B' hB' hBB' ↦ hB₁ ⟨hB', empty_subset _,h_support B' hB'⟩ hBB'⟩⟩ )
@@ -680,15 +692,15 @@ def Matroid_of_Indep (E : Set α) (Indep : Set α → Prop) (h_empty : Indep ∅
       exact hJmax (h_subset hBi' hB'') hIA hAX hJA ) 
   ( fun B hB ↦ h_support B hB.1 )
 
-@[simp] lemma Matroid_of_Indep_apply (E : Set α) (Indep : Set α → Prop) (h_empty : Indep ∅) 
+@[simp] theorem matroid_of_indep_apply (E : Set α) (Indep : Set α → Prop) (h_empty : Indep ∅) 
     (h_subset : ∀ ⦃I J⦄, Indep J → I ⊆ J → Indep I) 
     (h_aug : ∀⦃I B⦄, Indep I → I ∉ maximals (· ⊆ ·) Indep → B ∈ maximals (· ⊆ ·) Indep → 
       ∃ x ∈ B \ I, Indep (insert x I))
     (h_maximal : ∀ X, X ⊆ E → exists_maximal_subset_property Indep X) 
     (h_support : ∀ I, Indep I → I ⊆ E) : 
-    (Matroid_of_Indep E Indep h_empty h_subset h_aug h_maximal h_support).Indep = Indep := by
+    (matroid_of_indep E Indep h_empty h_subset h_aug h_maximal h_support).Indep = Indep := by
   ext I
-  simp_rw [Indep_iff_subset_Base, Matroid_of_Indep, Matroid_of_Base_apply, mem_maximals_Prop_iff]
+  simp_rw [indep_iff_subset_base, matroid_of_indep, matroid_of_base_apply, mem_maximals_Prop_iff]
   refine' ⟨fun ⟨B, ⟨hBi, _⟩, hIB⟩ ↦ h_subset hBi hIB, fun h ↦ _⟩
   obtain ⟨B, hB⟩ := h_maximal E rfl.subset I h (h_support I h)
   simp_rw [mem_maximals_setOf_iff, and_imp] at hB
@@ -702,7 +714,7 @@ theorem Matroid.exists_maximal_subset_property_of_bdd {P : Set α → Prop}
   simp_rw [encard_le_coe_iff] at hP
   rintro I hI hIX
   have hfin : Set.Finite (ncard '' {Y | P Y ∧ I ⊆ Y ∧ Y ⊆ X})
-  · rw [Finite_iff_BddAbove, bddAbove_def]
+  · rw [finite_iff_bddAbove, bddAbove_def]
     use n
     rintro x ⟨Y, ⟨hY,-,-⟩, rfl⟩
     exact (hP Y hY).2
@@ -712,47 +724,47 @@ theorem Matroid.exists_maximal_subset_property_of_bdd {P : Set α → Prop}
   refine' (eq_of_subset_of_ncard_le hYJ _ hJfin).symm.subset
   rw [hY' J ⟨hJ, hIJ, hJX⟩ (ncard_le_of_subset hYJ hJfin)]
 
-/-- If there is an absolute upper bound on the size of an Independent set, then the maximality axiom 
-  isn't needed to define a matroid by Independent sets. -/
-def Matroid_of_Indep_of_bdd (E : Set α) (Indep : Set α → Prop) (h_empty : Indep ∅) 
+/-- If there is an absolute upper bound on the size of an independent set, then the maximality axiom 
+  isn't needed to define a matroid by independent sets. -/
+def matroid_of_indep_of_bdd (E : Set α) (Indep : Set α → Prop) (h_empty : Indep ∅) 
     (h_subset : ∀ ⦃I J⦄, Indep J → I ⊆ J → Indep I) 
     (h_aug : ∀⦃I B⦄, Indep I → I ∉ maximals (· ⊆ ·) Indep → B ∈ maximals (· ⊆ ·) Indep → 
       ∃ x ∈ B \ I, Indep (insert x I))
     (h_bdd : ∃ (n : ℕ), ∀ I, Indep I → I.encard ≤ n )
     (h_support : ∀ I, Indep I → I ⊆ E) : Matroid α :=
-  Matroid_of_Indep E Indep h_empty h_subset h_aug 
+  matroid_of_indep E Indep h_empty h_subset h_aug 
     (fun X _ ↦ Matroid.exists_maximal_subset_property_of_bdd h_bdd X) h_support 
 
-@[simp] theorem Matroid_of_Indep_of_bdd_apply (E : Set α) (Indep : Set α → Prop) (h_empty : Indep ∅) 
+@[simp] theorem matroid_of_indep_of_bdd_apply (E : Set α) (Indep : Set α → Prop) (h_empty : Indep ∅) 
     (h_subset : ∀ ⦃I J⦄, Indep J → I ⊆ J → Indep I) 
     (h_aug : ∀⦃I B⦄, Indep I → I ∉ maximals (· ⊆ ·) Indep → B ∈ maximals (· ⊆ ·) Indep → 
       ∃ x ∈ B \ I, Indep (insert x I))
     (h_bdd : ∃ (n : ℕ), ∀ I, Indep I → I.encard ≤ n) (h_support : ∀ I, Indep I → I ⊆ E) : 
-    (Matroid_of_Indep_of_bdd E Indep h_empty h_subset h_aug h_bdd h_support).Indep = Indep := by
-  simp [Matroid_of_Indep_of_bdd]
+    (matroid_of_indep_of_bdd E Indep h_empty h_subset h_aug h_bdd h_support).Indep = Indep := by
+  simp [matroid_of_indep_of_bdd]
 
-/-- `Matroid_of_Indep_of_bdd` constructs a `Finite_rk` matroid. -/
+/-- `matroid_of_indep_of_bdd` constructs a `FiniteRk` matroid. -/
 instance (E : Set α) (Indep : Set α → Prop) (h_empty : Indep ∅) 
     (h_subset : ∀ ⦃I J⦄, Indep J → I ⊆ J → Indep I) 
     (h_aug : ∀⦃I B⦄, Indep I → I ∉ maximals (· ⊆ ·) Indep → B ∈ maximals (· ⊆ ·) Indep → 
       ∃ x ∈ B \ I, Indep (insert x I)) (h_bdd : ∃ (n : ℕ), ∀ I, Indep I → I.encard ≤ n ) 
     (h_support : ∀ I, Indep I → I ⊆ E) : 
-    Matroid.Finite_rk (Matroid_of_Indep_of_bdd E Indep h_empty h_subset h_aug h_bdd h_support) := by
+    Matroid.FiniteRk (matroid_of_indep_of_bdd E Indep h_empty h_subset h_aug h_bdd h_support) := by
   obtain ⟨B, hB⟩ := 
-    (Matroid_of_Indep_of_bdd E Indep h_empty h_subset h_aug h_bdd h_support).exists_Base
+    (matroid_of_indep_of_bdd E Indep h_empty h_subset h_aug h_bdd h_support).exists_base
   obtain ⟨n, h_bdd⟩ := h_bdd
   simp_rw [encard_le_coe_iff] at h_bdd
-  refine' hB.Finite_rk_of_Finite (h_bdd B _).1
-  rw [←Matroid_of_Indep_of_bdd_apply E Indep, Matroid.Indep]
+  refine' hB.finiteRk_of_finite (h_bdd B _).1
+  rw [←matroid_of_indep_of_bdd_apply E Indep, Matroid.Indep]
   exact ⟨_, hB, rfl.subset⟩
 
-def Matroid_of_Indep_of_bdd_augment (E : Set α) (Indep : Set α → Prop) (h_empty : Indep ∅) 
+def matroid_of_indep_of_bdd_augment (E : Set α) (Indep : Set α → Prop) (h_empty : Indep ∅) 
     (h_subset : ∀ ⦃I J⦄, Indep J → I ⊆ J → Indep I) 
     (ind_aug : ∀ ⦃I J⦄, Indep I → Indep J → I.ncard < J.ncard →
       ∃ e ∈ J, e ∉ I ∧ Indep (insert e I)) 
     (h_bdd : ∃ (n : ℕ), ∀ I, Indep I → I.encard ≤ n ) (h_support : ∀ I, Indep I → I ⊆ E) : 
     Matroid α := 
-  Matroid_of_Indep_of_bdd E Indep h_empty h_subset 
+  matroid_of_indep_of_bdd E Indep h_empty h_subset 
     (by {
       simp_rw [mem_maximals_Prop_iff, not_and, not_forall, exists_prop, exists_and_left, mem_diff,
         and_imp, and_assoc]
@@ -768,99 +780,99 @@ def Matroid_of_Indep_of_bdd_augment (E : Set α) (Indep : Set α → Prop) (h_em
       exact ind_aug hI hB (hlt.trans_le hle) })
     h_bdd h_support 
 
-@[simp] lemma Matroid_of_Indep_of_bbd_augment_apply (E : Set α) (Indep : Set α → Prop) 
+@[simp] theorem matroid_of_indep_of_bbd_augment_apply (E : Set α) (Indep : Set α → Prop) 
     (h_empty : Indep ∅) (h_subset : ∀ ⦃I J⦄, Indep J → I ⊆ J → Indep I) 
     (ind_aug : ∀ ⦃I J⦄, Indep I → Indep J → I.ncard < J.ncard →
       ∃ e ∈ J, e ∉ I ∧ Indep (insert e I)) 
     (h_bdd : ∃ (n : ℕ), ∀ I, Indep I → I.encard ≤ n ) (h_support : ∀ I, Indep I → I ⊆ E) : 
-    (Matroid_of_Indep_of_bdd_augment E Indep h_empty h_subset ind_aug h_bdd h_support).Indep 
+    (matroid_of_indep_of_bdd_augment E Indep h_empty h_subset ind_aug h_bdd h_support).Indep 
       = Indep := by
-  simp [Matroid_of_Indep_of_bdd_augment]
+  simp [matroid_of_indep_of_bdd_augment]
 
 /-- A collection of Bases with the exchange property and at least one finite member is a matroid -/
-def Matroid_of_exists_finite_Base {α : Type _} (E : Set α) (Base : Set α → Prop) 
-    (exists_finite_Base : ∃ B, Base B ∧ B.Finite) (Base_exchange : exchange_property Base) 
+def matroid_of_exists_finite_base {α : Type _} (E : Set α) (Base : Set α → Prop) 
+    (exists_finite_base : ∃ B, Base B ∧ B.Finite) (base_exchange : exchange_property Base) 
     (support : ∀ B, Base B → B ⊆ E) : Matroid α := 
-  Matroid_of_Base E Base 
-    (by { obtain ⟨B,h⟩ := exists_finite_Base; exact ⟨B,h.1⟩ }) Base_exchange 
+  matroid_of_base E Base 
+    (by { obtain ⟨B,h⟩ := exists_finite_base; exact ⟨B,h.1⟩ }) base_exchange 
     (by {
-      obtain ⟨B, hB, hfin⟩ := exists_finite_Base
+      obtain ⟨B, hB, hfin⟩ := exists_finite_base
       refine' fun X _ ↦ Matroid.exists_maximal_subset_property_of_bdd 
         ⟨B.ncard, fun Y ⟨B', hB', hYB'⟩ ↦ _⟩ X
-      rw [←hfin.encard_eq, encard_Base_eq_of_exch Base_exchange hB hB']
+      rw [←hfin.encard_eq, encard_base_eq_of_exch base_exchange hB hB']
       exact encard_mono hYB' })
     support
 
-@[simp] theorem Matroid_of_exists_finite_Base_apply {α : Type _} (E : Set α) (Base : Set α → Prop) 
-    (exists_finite_Base : ∃ B, Base B ∧ B.Finite) (Base_exchange : exchange_property Base) 
+@[simp] theorem matroid_of_exists_finite_base_apply {α : Type _} (E : Set α) (Base : Set α → Prop) 
+    (exists_finite_base : ∃ B, Base B ∧ B.Finite) (base_exchange : exchange_property Base) 
     (support : ∀ B, Base B → B ⊆ E) : 
-    (Matroid_of_exists_finite_Base E Base exists_finite_Base Base_exchange support).Base = Base := 
+    (matroid_of_exists_finite_base E Base exists_finite_base base_exchange support).Base = Base := 
   rfl 
 
-/-- A matroid constructed with a finite Base is `Finite_rk` -/
-instance {E : Set α} {Base : Set α → Prop} {exists_finite_Base : ∃ B, Base B ∧ B.Finite} 
-    {Base_exchange : exchange_property Base} {support : ∀ B, Base B → B ⊆ E} : 
-    Matroid.Finite_rk 
-      (Matroid_of_exists_finite_Base E Base exists_finite_Base Base_exchange support) := 
-  ⟨exists_finite_Base⟩  
+/-- A matroid constructed with a finite Base is `FiniteRk` -/
+instance {E : Set α} {Base : Set α → Prop} {exists_finite_base : ∃ B, Base B ∧ B.Finite} 
+    {base_exchange : exchange_property Base} {support : ∀ B, Base B → B ⊆ E} : 
+    Matroid.FiniteRk 
+      (matroid_of_exists_finite_base E Base exists_finite_base base_exchange support) := 
+  ⟨exists_finite_base⟩  
 
-def Matroid_of_Base_of_finite {E : Set α} (hE : E.Finite) (Base : Set α → Prop)
-    (exists_Base : ∃ B, Base B) (Base_exchange : exchange_property Base)
+def matroid_of_base_of_finite {E : Set α} (hE : E.Finite) (Base : Set α → Prop)
+    (exists_base : ∃ B, Base B) (base_exchange : exchange_property Base)
     (support : ∀ B, Base B → B ⊆ E) : Matroid α :=
-  Matroid_of_exists_finite_Base E Base 
-    (by { obtain ⟨B,hB⟩ := exists_Base; exact ⟨B,hB, hE.subset (support _ hB)⟩ }) 
-    Base_exchange support
+  matroid_of_exists_finite_base E Base 
+    (by { obtain ⟨B,hB⟩ := exists_base; exact ⟨B,hB, hE.subset (support _ hB)⟩ }) 
+    base_exchange support
 
-@[simp] theorem Matroid_of_Base_of_finite_apply {E : Set α} (hE : E.Finite) (Base : Set α → Prop)
-    (exists_Base : ∃ B, Base B) (Base_exchange : exchange_property Base)
+@[simp] theorem matroid_of_base_of_finite_apply {E : Set α} (hE : E.Finite) (Base : Set α → Prop)
+    (exists_base : ∃ B, Base B) (base_exchange : exchange_property Base)
     (support : ∀ B, Base B → B ⊆ E) : 
-    (Matroid_of_Base_of_finite hE Base exists_Base Base_exchange support).Base = Base := rfl 
+    (matroid_of_base_of_finite hE Base exists_base base_exchange support).Base = Base := rfl 
 
-/-- A collection of subsets of a finite ground set satisfying the usual Independence axioms 
+/-- A collection of subsets of a finite ground set satisfying the usual independence axioms 
   determines a matroid -/
-def Matroid_of_Indep_of_Finite {E : Set α} (hE : E.Finite) (Indep : Set α → Prop)
+def matroid_of_indep_of_finite {E : Set α} (hE : E.Finite) (Indep : Set α → Prop)
     (h_empty : Indep ∅)
     (ind_mono : ∀ ⦃I J⦄, Indep J → I ⊆ J → Indep I)
     (ind_aug : ∀ ⦃I J⦄, Indep I → Indep J → I.ncard < J.ncard → ∃ e ∈ J, e ∉ I ∧ Indep (insert e I)) 
     (h_support : ∀ ⦃I⦄, Indep I → I ⊆ E) : Matroid α := 
-  Matroid_of_Indep_of_bdd_augment E Indep h_empty ind_mono ind_aug
+  matroid_of_indep_of_bdd_augment E Indep h_empty ind_mono ind_aug
   (⟨E.ncard, fun I hI ↦ by { rw [←hE.encard_eq]; exact encard_mono (h_support hI) }⟩ )
   h_support
 
-instance Matroid_of_Indep_of_Finite.Finite {E : Set α} (hE : E.Finite) (Indep : Set α → Prop)
+instance matroid_of_indep_of_finite.Finite {E : Set α} (hE : E.Finite) (Indep : Set α → Prop)
     (h_empty : Indep ∅)
     (ind_mono : ∀ ⦃I J⦄, Indep J → I ⊆ J → Indep I)
     (ind_aug : ∀ ⦃I J⦄, Indep I → Indep J → I.ncard < J.ncard → ∃ e ∈ J, e ∉ I ∧ Indep (insert e I)) 
     (h_support : ∀ ⦃I⦄, Indep I → I ⊆ E) : 
-    ((Matroid_of_Indep_of_Finite) hE Indep h_empty ind_mono ind_aug h_support).Finite := 
+    ((matroid_of_indep_of_finite) hE Indep h_empty ind_mono ind_aug h_support).Finite := 
   ⟨hE⟩ 
 
-instance Matroid_of_Indep_of_Finite_apply {E : Set α} (hE : E.Finite) (Indep : Set α → Prop)
+instance matroid_of_indep_of_finite_apply {E : Set α} (hE : E.Finite) (Indep : Set α → Prop)
     (h_empty : Indep ∅)
     (ind_mono : ∀ ⦃I J⦄, Indep J → I ⊆ J → Indep I)
     (ind_aug : ∀ ⦃I J⦄, Indep I → Indep J → I.ncard < J.ncard → ∃ e ∈ J, e ∉ I ∧ Indep (insert e I)) 
     (h_support : ∀ ⦃I⦄, Indep I → I ⊆ E) : 
-    ((Matroid_of_Indep_of_Finite) hE Indep h_empty ind_mono ind_aug h_support).Indep = Indep := by
-  simp [Matroid_of_Indep_of_Finite]
+    ((matroid_of_indep_of_finite) hE Indep h_empty ind_mono ind_aug h_support).Indep = Indep := by
+  simp [matroid_of_indep_of_finite]
 
 end from_axioms
 
 section dual 
 
-def Dual (M : Matroid α) : Matroid α := 
-  Matroid_of_Indep M.E (fun I ↦ I ⊆ M.E ∧ ∃ B, M.Base B ∧ Disjoint I B) 
-⟨empty_subset M.E, M.exists_Base.imp (fun B hB ↦ ⟨hB, empty_disjoint _⟩)⟩ 
+def dual (M : Matroid α) : Matroid α := 
+  matroid_of_indep M.E (fun I ↦ I ⊆ M.E ∧ ∃ B, M.Base B ∧ Disjoint I B) 
+⟨empty_subset M.E, M.exists_base.imp (fun B hB ↦ ⟨hB, empty_disjoint _⟩)⟩ 
 ( by { 
     rintro I J ⟨hJE, B, hB, hJB⟩ hIJ
     exact ⟨hIJ.trans hJE, ⟨B, hB, disjoint_of_subset_left hIJ hJB⟩⟩ } )
 ( by { 
     rintro I X ⟨hIE, B, hB, hIB⟩ hI_not_max hX_max
     have hXE := hX_max.1.1
-    have hB' := (Base_compl_iff_mem_maximals_disjoint_Base hXE).mpr hX_max
+    have hB' := (base_compl_iff_mem_maximals_disjoint_base hXE).mpr hX_max
     
     set B' := M.E \ X with hX
-    have hI := (not_iff_not.mpr (Base_compl_iff_mem_maximals_disjoint_Base)).mpr hI_not_max
-    obtain ⟨B'', hB'', hB''₁, hB''₂⟩ := (hB'.Indep.diff I).exists_Base_subset_union_Base hB 
+    have hI := (not_iff_not.mpr (base_compl_iff_mem_maximals_disjoint_base)).mpr hI_not_max
+    obtain ⟨B'', hB'', hB''₁, hB''₂⟩ := (hB'.indep.diff I).exists_base_subset_union_base hB 
     rw [←compl_subset_compl, ←hIB.sdiff_eq_right, ←union_diff_distrib, diff_eq, compl_inter, 
       compl_compl, union_subset_iff, compl_subset_compl] at hB''₂ 
     
@@ -876,8 +888,8 @@ def Dual (M : Matroid α) : Matroid α :=
     exact disjoint_of_subset_left hB''₂.2 disjoint_compl_left } ) 
 ( by {
     rintro X - I'⟨hI'E, B, hB, hI'B⟩ hI'X
-    obtain ⟨I, hI⟩ :=  M.exists_Basis (M.E \ X)
-    obtain ⟨B', hB', hIB', hB'IB⟩ := hI.Indep.exists_Base_subset_union_Base hB
+    obtain ⟨I, hI⟩ :=  M.exists_basis (M.E \ X)
+    obtain ⟨B', hB', hIB', hB'IB⟩ := hI.indep.exists_base_subset_union_base hB
     refine' ⟨(X \ B') ∩ M.E, 
       ⟨_,subset_inter (subset_diff.mpr _) hI'E, (inter_subset_left _ _).trans (diff_subset _ _)⟩, _⟩ 
     · simp only [inter_subset_right, true_and]
@@ -899,15 +911,15 @@ def Dual (M : Matroid α) : Matroid α :=
            _ ⊆ _ := by rw [inter_distrib_left, hdj.symm.inter_eq, union_empty] 
            _ ⊆ _ := inter_subset_right _ _
     
-    obtain ⟨B₁,hB₁,hI'B₁,hB₁I⟩ := (hB'.Indep.subset hI').exists_Base_subset_union_Base hB''
+    obtain ⟨B₁,hB₁,hI'B₁,hB₁I⟩ := (hB'.indep.subset hI').exists_base_subset_union_base hB''
     rw [union_comm, ←union_assoc, union_eq_self_of_subset_right (inter_subset_left _ _)] at hB₁I
     
     have : B₁ = B'
-    · refine' hB₁.eq_of_subset_Indep hB'.Indep (fun e he ↦ _)
+    · refine' hB₁.eq_of_subset_indep hB'.indep (fun e he ↦ _)
       refine' (hB₁I he).elim (fun heB'' ↦ _) (fun h ↦ h.1)
       refine' (em (e ∈ X)).elim (fun heX ↦ hI' (Or.inl ⟨heB'', heX⟩)) (fun heX ↦ hIB' _)
-      refine' hI.mem_of_insert_Indep ⟨hB₁.subset_ground he, heX⟩ 
-        (hB₁.Indep.subset (insert_subset.mpr ⟨he, _⟩))
+      refine' hI.mem_of_insert_indep ⟨hB₁.subset_ground he, heX⟩ 
+        (hB₁.indep.subset (insert_subset.mpr ⟨he, _⟩))
       refine' (subset_union_of_subset_right (subset_diff.mpr ⟨hIB',_⟩) _).trans hI'B₁
       refine' disjoint_of_subset_left hI.subset disjoint_sdiff_left 
 
@@ -920,137 +932,282 @@ def Dual (M : Matroid α) : Matroid α :=
     exact heX (hJX heJ) } ) 
 ( by tauto )  
 
+/-- A notation typeclass for matroid duality, denoted by the `*` symbol. -/
+class Mdual (β : Type _) := (dual : β → β)
 
-/-- A notation typeclass for matroid duality, denoted by the `﹡` symbol. -/
-class MDual (β : Type _) := (Dual : β → β)
+postfix:max "*" => Mdual.dual
 
-postfix:max "*" => MDual.Dual
+instance Matroid_Mdual {α : Type _} : Mdual (Matroid α) := ⟨Matroid.dual⟩ 
 
-instance Matroid_MDual {α : Type _} : MDual (Matroid α) := ⟨Matroid.Dual⟩ 
+theorem dual_indep_iff_exists' : ((M*).Indep I) ↔ I ⊆ M.E ∧ (∃ B, M.Base B ∧ Disjoint I B) := 
+  by simp [Mdual.dual, dual]
 
-theorem Dual_Indep_iff_exists' : ((M*).Indep I) ↔ I ⊆ M.E ∧ (∃ B, M.Base B ∧ Disjoint I B) := 
-  by simp [MDual.Dual, Dual]
+@[simp] theorem dual_ground : (M*).E = M.E := rfl 
 
-@[simp] theorem Dual_ground : (M*).E = M.E := rfl 
+@[aesop unsafe 10% (rule_sets [Matroid])]
+theorem subset_dual_ground_of_subset_ground (hX : X ⊆ M.E) : X ⊆ (M*).E :=
+  hX 
 
-@[simp] theorem Dual_Indep_iff_exists (hI : I ⊆ M.E := by aesop_mat) : 
+@[aesop unsafe 10% (rule_sets [Matroid])]
+theorem subset_ground_of_subset_dual_ground (hX : X ⊆ (M*).E) : X ⊆ M.E :=
+  hX 
+
+@[simp] theorem dual_indep_iff_exists (hI : I ⊆ M.E := by aesop_mat) : 
   ((M*).Indep I) ↔ (∃ B, M.Base B ∧ Disjoint I B) := 
-by rw [Dual_Indep_iff_exists', and_iff_right hI]
+by rw [dual_indep_iff_exists', and_iff_right hI]
 
-theorem Dual_Dep_iff_forall : ((M*).Dep I) ↔ (∀ B, M.Base B → (I ∩ B).Nonempty) ∧ I ⊆ M.E := 
-  by simp_rw [Dep_iff, Dual_Indep_iff_exists', Dual_ground, and_congr_left_iff, not_and, 
+theorem dual_dep_iff_forall : ((M*).Dep I) ↔ (∀ B, M.Base B → (I ∩ B).Nonempty) ∧ I ⊆ M.E := 
+  by simp_rw [dep_iff, dual_indep_iff_exists', dual_ground, and_congr_left_iff, not_and, 
     not_exists, not_and, not_disjoint_iff_nonempty_inter, imp_iff_right_iff, iff_true_intro Or.inl]
   
 instance dual_finite [M.Finite] : (M*).Finite := 
-  ⟨M.ground_Finite⟩  
+  ⟨M.ground_finite⟩  
 
-theorem subset_ground_Dual (hX : X ⊆ M.E := by aesop_mat) : X ⊆ (M*).E := 
+theorem subset_ground_dual (hX : X ⊆ M.E := by aesop_mat) : X ⊆ (M*).E := 
   hX 
 
-theorem Dual_Base_iff (hB : B ⊆ M.E := by aesop_mat) : (M*).Base B ↔ M.Base (M.E \ B) := by
-  rw [Base_compl_iff_mem_maximals_disjoint_Base, Base_iff_maximal_Indep, Dual_Indep_iff_exists', 
+@[simp] theorem dual_base_iff (hB : B ⊆ M.E := by aesop_mat) : (M*).Base B ↔ M.Base (M.E \ B) := by
+  rw [base_compl_iff_mem_maximals_disjoint_base, base_iff_maximal_indep, dual_indep_iff_exists', 
     mem_maximals_setOf_iff]
-  simp [Dual_Indep_iff_exists']
+  simp [dual_indep_iff_exists']
 
-theorem Dual_Base_iff' : (M*).Base B ↔ M.Base (M.E \ B) ∧ B ⊆ M.E :=
-  (em (B ⊆ M.E)).elim (fun h ↦ by rw [Dual_Base_iff, and_iff_left h]) 
+theorem dual_base_iff' : (M*).Base B ↔ M.Base (M.E \ B) ∧ B ⊆ M.E :=
+  (em (B ⊆ M.E)).elim (fun h ↦ by rw [dual_base_iff, and_iff_left h]) 
     (fun h ↦ iff_of_false (h ∘ (fun h' ↦ h'.subset_ground)) (h ∘ And.right))
 
-theorem Base.compl_Base_Dual (h : (M*).Base B) : M.Base (M.E \ B) := 
-  (Dual_Base_iff'.1 h).1
+@[simp] theorem dual_dual (M : Matroid α) : M** = M :=  
+  eq_of_base_iff_base_forall rfl (fun B (h : B ⊆ M.E) ↦ 
+    by rw [dual_base_iff, dual_base_iff, dual_ground, diff_diff_cancel_left h])
 
-@[simp] theorem Dual_Dual (M : Matroid α) : M** = M :=  
-  eq_of_Base_iff_Base_forall rfl (fun B (h : B ⊆ M.E) ↦ 
-    by rw [Dual_Base_iff, Dual_Base_iff, Dual_ground, diff_diff_cancel_left h])
+theorem Base.compl_base_of_dual (h : (M*).Base B) : M.Base (M.E \ B) := 
+  (dual_base_iff'.1 h).1
 
-theorem dual_Indep_iff_Coindep : (M*).Indep X ↔ M.Coindep X := by 
-  rw [Dual_Indep_iff_exists', and_comm]; rfl
+theorem Base.compl_base_dual (h : M.Base B) : (M*).Base (M.E \ B) := by
+  rwa [dual_base_iff, diff_diff_cancel_left h.subset_ground] 
 
-theorem Base.compl_inter_Basis_of_inter_Basis (hB : M.Base B) (hBX : M.Basis (B ∩ X) X) :
+@[simp] theorem dual_indep_iff_Coindep : (M*).Indep X ↔ M.Coindep X := by 
+  rw [dual_indep_iff_exists', and_comm]; rfl
+
+theorem Base.compl_inter_basis_of_inter_basis (hB : M.Base B) (hBX : M.Basis (B ∩ X) X) :
     (M*).Basis ((M.E \ B) ∩ (M.E \ X)) (M.E \ X) := by
-  refine' Indep.Basis_of_forall_insert _ (inter_subset_right _ _) (fun e he ↦ _)
-  · rw [Dual_Indep_iff_exists]
+  refine' Indep.basis_of_forall_insert _ (inter_subset_right _ _) (fun e he ↦ _)
+  · rw [dual_indep_iff_exists]
     exact ⟨B, hB, disjoint_of_subset_left (inter_subset_left _ _) disjoint_sdiff_left⟩
   simp only [diff_inter_self_eq_diff, mem_diff, not_and, not_not, imp_iff_right he.1.1] at he 
-  simp_rw [Dual_Dep_iff_forall, insert_subset, and_iff_right he.1.1, 
+  simp_rw [dual_dep_iff_forall, insert_subset, and_iff_right he.1.1, 
     and_iff_left ((inter_subset_left _ _).trans (diff_subset _ _))]
   refine' fun B' hB' ↦ by_contra (fun hem ↦ _)
-  rw [nonempty_iff_ne_empty, not_ne_iff, ←union_singleton, inter_distrib_right, 
-    union_empty_iff] at hem
+  simp_rw [nonempty_iff_ne_empty, not_ne_iff, ←union_singleton, inter_distrib_right, 
+    union_empty_iff, singleton_inter_eq_empty, diff_eq, inter_comm _ M.E, 
+    ←inter_inter_distrib_left, ← inter_assoc, inter_right_comm, 
+    inter_eq_self_of_subset_right hB'.subset_ground, ←diff_eq, diff_eq_empty] at hem
+  obtain ⟨f, hfb, hBf⟩ := hB.exchange hB' ⟨he.2, hem.2⟩ 
   
+  have hi : M.Indep (insert f (B ∩ X))
+  · refine' hBf.indep.subset (insert_subset_insert _)
+    simp_rw [subset_diff, and_iff_right (inter_subset_left _ _), disjoint_singleton_right, 
+      mem_inter_iff, iff_false_intro he.1.2, and_false]
+  exact hfb.2 (hBX.mem_of_insert_indep (hem.1 hfb) hi).1 
 
+theorem Base.inter_basis_iff_compl_inter_basis_dual (hB : M.Base B) (hX : X ⊆ M.E := by aesop_mat): 
+    M.Basis (B ∩ X) X ↔ (M*).Basis ((M.E \ B) ∩ (M.E \ X)) (M.E \ X) := by
+  refine' ⟨hB.compl_inter_basis_of_inter_basis, fun h ↦ _⟩
+  simpa [inter_eq_self_of_subset_right hX, inter_eq_self_of_subset_right hB.subset_ground] using
+    hB.compl_base_dual.compl_inter_basis_of_inter_basis h
+    
+theorem dual_inj {M₁ M₂ : Matroid α} (h : M₁* = M₂*) : M₁ = M₂ :=
+by rw [←dual_dual M₁, h, dual_dual]
 
+@[simp] theorem dual_inj_iff {M₁ M₂ : Matroid α} : M₁* = M₂* ↔ M₁ = M₂ := ⟨dual_inj, congr_arg _⟩
+
+theorem eq_dual_comm {M₁ M₂ : Matroid α} : M₁ = M₂* ↔ M₂ = M₁* := 
+by rw [←dual_inj_iff, dual_dual, eq_comm]
+
+theorem dual_eq_comm {M₁ M₂ : Matroid α} : M₁* = M₂ ↔ M₂* = M₁ := 
+by rw [←dual_inj_iff, dual_dual, eq_comm]
+
+theorem base_iff_dual_base_compl (hB : B ⊆ M.E := by aesop_mat) :
+    M.Base B ↔ (M*).Base (M.E \ B) := by 
+  rw [dual_base_iff, diff_diff_cancel_left hB]
 
 end dual 
+
+section restrict
+
+/-- Restrict the matroid `M` to `X : Set α`.  -/
+def Restrict (M : Matroid α) (X : Set α) : Matroid α :=
+matroid_of_indep (X ∩ M.E) (fun I ↦ M.Indep I ∧ I ⊆ X ∩ M.E) ⟨M.empty_indep, empty_subset _⟩ 
+(fun I J hJ hIJ ↦ ⟨hJ.1.subset hIJ, hIJ.trans hJ.2⟩)
+(by {
+  set Y := X ∩ M.E
+  have hY : Y ⊆ M.E := inter_subset_right _ _ 
+  rintro I I' ⟨hI, hIY⟩ hIn hI'
+  rw [←basis_iff_mem_maximals_Prop] at hIn hI'
+
+  obtain ⟨B', hB', rfl⟩ := hI'.exists_base
+  obtain ⟨B, hB, hIB, hBIB'⟩ := hI.exists_base_subset_union_base hB'
+  
+  rw [hB'.inter_basis_iff_compl_inter_basis_dual hY, diff_inter_diff] at hI'
+  
+  have hss : M.E \ (B' ∪ Y) ⊆ M.E \ (B ∪ Y)
+  · rw [subset_diff, and_iff_right (diff_subset _ _), ←subset_compl_iff_disjoint_left, 
+      diff_eq, compl_inter, compl_compl, ←union_assoc, union_subset_iff, 
+      and_iff_left (subset_union_right _ _)]
+    refine hBIB'.trans (union_subset (hIY.trans ?_) 
+      (subset_union_of_subset_left (subset_union_right _ _) _))
+    apply subset_union_right
+
+  have hi : (M*).Indep (M.E \ (B ∪ Y))
+  · rw [dual_indep_iff_Coindep, coindep_iff_exists, 
+      diff_diff_cancel_left (union_subset hB.subset_ground hY)]
+    exact ⟨B, hB, subset_union_left _ _⟩ 
+
+  have h_eq := hI'.eq_of_subset_indep hi hss 
+    (by {rw [diff_subset_iff, union_assoc, union_diff_self, ←union_assoc]; simp })
+  
+  rw [h_eq, ←diff_inter_diff, ←hB.inter_basis_iff_compl_inter_basis_dual hY] at hI'
+
+  have hssu : I ⊂ (B ∩ Y) := (subset_inter hIB hIY).ssubset_of_ne 
+    (by { rintro rfl; exact hIn hI' })
+
+  obtain ⟨e, heBY, heI⟩ := exists_of_ssubset hssu
+  exact ⟨e, ⟨⟨(hBIB' heBY.1).elim (fun h' ↦  (heI h').elim) id ,heBY.2⟩,heI⟩, 
+    (hB.indep.inter_right Y).subset (insert_subset.mpr ⟨heBY,hssu.subset⟩), 
+    insert_subset.mpr ⟨heBY.2,hssu.subset.trans (inter_subset_right _ _)⟩⟩ })
+(by {
+  rintro A hAE I ⟨hI, hIX⟩ hIA
+  obtain ⟨J, hJ, hIJ⟩ := hI.subset_basis_of_subset (subset_inter hIA hIX)
+  refine' ⟨J, ⟨⟨hJ.indep,hJ.subset.trans (inter_subset_right _ _)⟩,hIJ,
+    hJ.subset.trans (inter_subset_left _ _)⟩, fun B hB hJB ↦ _⟩
+  rw [hJ.eq_of_subset_indep hB.1.1 hJB (subset_inter hB.2.2 hB.1.2)]
+  })
+( by tauto )   
+
+variable {R R₁ R₂ : Set α}
+
+class MRestrict (α β : Type _) := (restrict : α → β → α)
+
+infixl:65  " | " => MRestrict.restrict
+
+instance {α : Type _} : MRestrict (Matroid α) (Set α) := ⟨fun M X ↦ M.Restrict X⟩  
+
+@[simp] theorem restrict_indep_iff : (M | R).Indep I ↔ M.Indep I ∧ I ⊆ R := by
+  change (M.Restrict R).Indep I ↔ _
+  simp only [Restrict, subset_inter_iff, matroid_of_indep_apply, and_congr_right_iff, 
+    and_iff_left_iff_imp]
+  exact fun h _ ↦ h.subset_ground
+
+theorem Indep.indep_restrict_of_subset (h : M.Indep I) (hIR : I ⊆ R) : (M | R).Indep I := 
+  restrict_indep_iff.mpr ⟨h,hIR⟩
+
+theorem restrict_ground_eq' : (M | R).E = R ∩ M.E := rfl 
+
+@[simp] theorem restrict_ground_eq (hR : R ⊆ M.E := by aesop_mat ) : (M | R).E = R := by
+  rwa [restrict_ground_eq', inter_eq_left_iff_subset]
+
+instance restrict_finite {R : Set α} [M.Finite] : (M | R).Finite := 
+  ⟨M.ground_finite.subset (inter_subset_right _ _)⟩  
+
+@[simp] theorem restrict_dep_iff : (M | R).Dep X ↔ M.Dep X ∧ X ⊆ R := by
+  rw [Dep, Dep, restrict_indep_iff, restrict_ground_eq', subset_inter_iff]; tauto
+
+@[simp] theorem restrict_ground_eq_self (M : Matroid α) : M | M.E = M := by
+  refine' eq_of_indep_iff_indep_forall (inter_self _) _
+  simp_rw [restrict_ground_eq']
+  aesop
+
+theorem restrict_eq_restrict_iff {R₁ R₂ : Set α} : M | R₁ = M | R₂ ↔ R₁ ∩ M.E = R₂ ∩ M.E := by
+  rw [eq_iff_indep_iff_indep_forall, restrict_ground_eq', restrict_ground_eq']
+  simp only [subset_inter_iff, restrict_indep_iff, and_congr_right_iff, and_imp, 
+    and_iff_left_iff_imp]
+  rintro h_eq I hIR₁ hIE -
+  rw [iff_true_intro hIR₁, true_iff]
+  exact ((subset_inter hIR₁ hIE).trans h_eq.subset).trans (inter_subset_left _ _)
+
+theorem restrict_inter_ground (M : Matroid α) (R : Set α) : M | (R ∩ M.E) = M | R := by
+  rw [restrict_eq_restrict_iff, inter_assoc, inter_self]
+
+theorem restrict_restrict (M : Matroid α) (R₁ R₂ : Set α) : (M | R₁) | R₂ = M | (R₁ ∩ R₂) :=
+  eq_of_indep_iff_indep_forall (by simp [restrict_ground_eq', ←inter_assoc, inter_comm R₁ R₂]) 
+    (by aesop)
+
+theorem restrict_restrict_of_subset (M : Matroid α) {R₁ R₂ : Set α} (hR : R₂ ⊆ R₁) :
+    (M | R₁) | R₂ = M | R₂ :=
+  by rw [restrict_restrict, inter_eq_self_of_subset_right hR]
+
+theorem Indep.of_restrict (hI : (M | R).Indep I) : M.Indep I := 
+  (restrict_indep_iff.mp hI).1 
+
+@[simp] theorem restrict_base_iff (hX : X ⊆ M.E := by aesop_mat) :
+    (M | X).Base I ↔ M.Basis I X := by
+  simp_rw [base_iff_maximal_indep, basis_iff', restrict_indep_iff, and_iff_left hX, and_assoc]
+  aesop
+  
+instance restrict_finiteRk [M.FiniteRk] : (M | R).FiniteRk := 
+  let ⟨_, hB⟩ := (M | R).exists_base
+  hB.finiteRk_of_finite (hB.indep.of_restrict.finite)
+
+@[simp] theorem basis.base_restrict (h : M.Basis I X) : (M | X).Base I := 
+  (restrict_base_iff h.subset_ground).mpr h
+
+theorem basis.basis_restrict_of_subset (hI : M.Basis I X) (hXY : X ⊆ Y) 
+    (hY : Y ⊆ M.E := by aesop_mat) : (M | Y).Basis I X := by
+  rwa [←restrict_base_iff, M.restrict_restrict_of_subset hXY, restrict_base_iff]
+
+theorem restrict_eq_self_iff : M | X = M ↔ M.E ⊆ X := by
+  simp only [eq_iff_indep_iff_indep_forall, restrict_indep_iff, and_iff_left_iff_imp, 
+    restrict_ground_eq', inter_eq_right_iff_subset]
+  exact fun _ I hI _ ↦ hI.trans (inter_subset_left _ _)
+
+def Restriction (N M : Matroid α) : Prop := M | N.E = N 
+
+def StrictRestriction (N M : Matroid α) : Prop := (M | N.E = N) ∧ N.E ⊂ M.E 
+
+infix:20  " ≤r " => Restriction
+infix:20  " <r " => StrictRestriction
+
+theorem Restriction.eq_restrict (h : N ≤r M) : M | N.E = N :=
+  h 
+
+theorem Restriction.ground_subset_ground (h : N ≤r M) : N.E ⊆ M.E := by
+  rw [←h.eq_restrict]; apply inter_subset_right 
+
+theorem Restriction.exists_eq_restrict (h : N ≤r M) : ∃ R, R ⊆ M.E ∧ N = M | R := by
+  rw [←h.eq_restrict]; exact ⟨N.E, h.ground_subset_ground, rfl⟩ 
+
+theorem StrictRestriction.restriction (h : N <r M) : N ≤r M :=
+  h.1
+
+@[simp] theorem restrict_restriction (M : Matroid α) (R : Set α) : M | R ≤r M := by
+  rw [Restriction, restrict_ground_eq', restrict_inter_ground]
+
+theorem StrictRestriction.Ne (h : N <r M) : N ≠ M := by
+  rintro rfl; exact h.2.ne rfl
+
+theorem Restriction.strictRestriction_of_ne (h : N ≤r M) (hne : N ≠ M) : N <r M := by
+  rw [StrictRestriction, and_iff_right h.eq_restrict, ssubset_iff_subset_ne, ←h.eq_restrict, 
+    restrict_ground_eq', and_iff_right (inter_subset_right _ _), Ne.def, inter_eq_right_iff_subset]
+  intro h_eq
+  rw [←h.eq_restrict, ←restrict_inter_ground, inter_eq_self_of_subset_right h_eq, 
+    restrict_ground_eq_self] at hne
+  exact hne rfl 
+
+instance Restriction.trans : IsTrans (Matroid α) (· ≤r ·) := 
+  ⟨fun M₁ M₂ M₃ h₁ h₂ ↦ by 
+  { rw [←h₁.eq_restrict, ←h₂.eq_restrict, Restriction]
+    simp_rw [restrict_ground_eq', restrict_restrict, restrict_eq_restrict_iff] 
+    rw [inter_assoc, inter_assoc, inter_self, inter_right_comm, inter_comm _ M₁.E] }⟩ 
+
+instance Restriction.refl : IsRefl (Matroid α) (· ≤r ·) := 
+  ⟨restrict_ground_eq_self⟩   
+
+instance Restriction.antisymm : IsAntisymm (Matroid α) (· ≤r ·) :=
+  ⟨fun M M' h h' ↦ by rw [←h.eq_restrict, h.ground_subset_ground.antisymm h'.ground_subset_ground,
+    restrict_ground_eq_self]⟩ 
+
+end restrict
 
 
 
 end Matroid 
 
-
-
-
-
--- 
-
--- theorem Base.compl_inter_Basis_of_inter_Basis (hB : M.Base B) (hBX : M.Basis (B ∩ X) X) :
---   M﹡.Basis ((M.E \ B) ∩ (M.E \ X)) (M.E \ X) := 
--- begin
---   rw Basis_iff, 
---   refine ⟨(hB.compl_Base_dual.Indep.subset (inter_subset_left _ _)), inter_subset_right _ _, 
---     λ J hJ hBCJ hJX, hBCJ.antisymm (subset_inter _ hJX)⟩, 
-  
---   obtain ⟨-, B', hB', hJB'⟩ := dual_Indep_iff_Coindep.mp hJ, 
-
---   obtain ⟨B'', hB'', hsB'', hB''s⟩  := hBX.Indep.exists_Base_subset_union_Base hB', 
---   have hB'ss : B' ⊆ B ∪ X, 
---   { rw [←diff_subset_diff_iff M.E (by ssE : B ∪ X ⊆ M.E) hB'.subset_ground, subset_diff,
---       and_iff_right (diff_subset _ _)],
---     rw [diff_inter_diff] at hBCJ, 
---     exact disjoint_of_subset_left hBCJ hJB' },
-  
---   have hB''ss : B'' ⊆ B, 
---   { refine λ e he, (hB''s he).elim and.left (λ heB', (hB'ss heB').elim id (λ heX, _)), 
---      exact (hBX.mem_of_insert_Indep heX (hB''.Indep.subset (insert_subset.mpr ⟨he,hsB''⟩))).1 }, 
-  
---   have := (hB''.eq_of_subset_Indep hB.Indep hB''ss).symm, subst this,
---   rw subset_diff at *, 
---   exact ⟨hJX.1, disjoint_of_subset_right hB''s (disjoint_union_right.mpr 
---     ⟨disjoint_of_subset_right (inter_subset_right _ _) hJX.2, hJB'⟩)⟩, 
--- end 
-
--- theorem Base.inter_Basis_iff_compl_inter_Basis_dual (hB : M.Base B) (hX : X ⊆ M.E := by aesop_mat): 
---   M.Basis (B ∩ X) X ↔ M﹡.Basis ((M.E \ B) ∩ (M.E \ X)) (M.E \ X) :=
--- begin
---   refine ⟨hB.compl_inter_Basis_of_inter_Basis, λ h, _⟩, 
---   simpa using hB.compl_Base_dual.compl_inter_Basis_of_inter_Basis h, 
--- end 
-  
--- theorem dual_inj {M₁ M₂ : Matroid α} (h : M₁﹡ = M₂﹡) : M₁ = M₂ :=
--- by rw [←dual_dual M₁, h, dual_dual]
-
--- @[simp] theorem dual_inj_iff {M₁ M₂ : Matroid α} : M₁﹡ = M₂﹡ ↔ M₁ = M₂ := ⟨dual_inj, congr_arg _⟩
-
--- theorem eq_dual_comm {M₁ M₂ : Matroid α} : M₁ = M₂﹡ ↔ M₂ = M₁﹡ := 
--- by rw [←dual_inj_iff, dual_dual, eq_comm]
-
--- theorem dual_eq_comm {M₁ M₂ : Matroid α} : M₁﹡ = M₂ ↔ M₂﹡ = M₁ := 
--- by rw [←dual_inj_iff, dual_dual, eq_comm]
-
--- theorem Coindep_iff_exists (hX : X ⊆ M.E := by aesop_mat) : M.Coindep X ↔ ∃ B, M.Base B ∧ disjoint X B := 
--- by rw [Coindep, and_iff_right hX]
-
--- theorem Coindep.exists_disjoint_Base (hX : M.Coindep X) : ∃ B, M.Base B ∧ disjoint X B := hX.2
-
--- theorem Coindep.Base_of_Basis_compl (hX : M.Coindep X) (hB : M.Basis B Xᶜ) : M.Base B :=
--- begin
---   obtain ⟨B',hB'⟩ := hX.exists_disjoint_Base, 
---   exact hB'.1.Base_of_Basis_supset (subset_compl_iff_disjoint_left.mpr hB'.2) hB, 
--- end 
-
--- theorem Base_iff_dual_Base_compl (hB : B ⊆ M.E := by aesop_mat) : M.Base B ↔ M﹡.Base (M.E \ B) :=
--- by simp [dual_Base_iff]
-
--- end dual 
-
--- end Matroid 
